Evaluation, reorg, lemmas
This is a bit of a monumental commit - there wasn't really a good point
to commit between then and now because of the scale of the reorg.

Unscoped.v has been broken into smaller pieces - now just exports the
core exp datatype, weakening, substitution, and some useful tactics for
using both of those

DeBrujin.v contains all the standard DeBrujin lifting / substitution lemmas
Scoping is where the scoping relation lives now, and lemmas having to do
with it (turns out we don't really use them anywhere else)

Anything having to do with the scoping relation has been moved to
Scoping.v

Evaluation.v contains a small step evaluation relation and a proof of
confluence. Right now the proof lives in Prop, but that shouldn't
matter when this is eventually moved to a theory without Prop.

Progress.v contains a proof of the progression property of arbitrary
terms, which /does/ hold computationally.

TypeChecking.v no longer quite lives up to its name. There's a lot of
work still to be done in here before that can be possible. In
particular, there's a lot of plumbing to deal with to finish the proof
of unique-typing-up-to-evaluation and normalization, the first of which
is necessary for typechecking right now.

I should note that this would all be helped by a theory with real
quotient types, but representing those might also be /difficult/.

coq-in-coq/TypeChecking.v
@@ -1,111 +1,447 @@
-Require Import Unscoped.
+(* imports *)
+Require Import Omega Coq.Program.Program Coq.Program.Tactics.
+Require Import Unscoped Scoping Evaluation.
+
+(* notations *)
+Open Scope list_scope.
 Infix "==" := (exp_eq_dec) (at level 50).
 
-Open Scope type_scope.
+(* Program things *)
+Set Shrink Obligations.
+Unset Transparent Obligations.
+Set Hide Obligations.
+Obligation Tactic := program_simpl; simpl in *; try omega.
 
-Definition and_sumor A1 A2 P1 P2 : A1 + {P1} -> A2 + {P2} -> (A1 * A2) + {P1 \/ P2}.
-  repeat destruct 1; auto. Defined.
+Set Implicit Arguments.
 
-Arguments and_sumor {A1} {A2} {P1} {P2} s1 s2.
-Infix "&&" := and_sumor.
+Fixpoint lookup_con {A} (Gamma: list A) (i : nat) : A + {i >= length Gamma} :=
+  match Gamma , i with
+    | nil , _ => inright (Peano.le_0_n i)
+    | (X :: Gamma) , 0 => inleft X
+    | (X :: Gamma) , S n => match lookup_con Gamma n with
+                         | inleft T => inleft T
+                         | inright p => inright (le_n_S _ _ p)
+                       end
+  end.
 
-Lemma typ_uq Gamma e T1 T2 : Gamma ⊢ e ∈ T1 -> Gamma ⊢ e ∈ T2 -> T1 = T2.
-  intro Ht1; generalize dependent T2; induction Ht1; inversion 1; subst; intros;
-  repeat match goal with [IH: forall T, ?Gamma ⊢ ?A ∈ T -> ?T1 = T, H : ?Gamma ⊢ ?A ∈ ?T2 |- _] => apply IH in H; inversion H; subst end;
-  try reflexivity.
-  - unfold lookup_wk; f_equal; apply lookup_irrel.
+Definition forget_prop {A P} : A + {P} -> option A. destruct 1; [left|right]; auto. Defined.
+
+Program Fixpoint lookup_lt {A} (Gamma : list A) (i : {x | x < length Gamma}) : A :=
+  match Gamma , i with
+    | nil , _ => False_rect _ _
+    | (x :: xs) , 0   => x
+    | (x :: xs) , S n => lookup_lt xs n
+  end.
+
+Lemma lookup_irrel A (Gamma : list A) : forall i j, `i = `j -> lookup_lt Gamma i = lookup_lt Gamma j.
+  induction Gamma; destruct i as [i Hi]; destruct j as [j Hj]; simpl in *; destruct 1; 
+  [exfalso; omega|destruct i]; eauto. Qed.
+
+Hint Rewrite lookup_irrel.
+
+Program Definition fsu {n} : {x | x < n} -> {x | x < S n} := S.
+
+Lemma lookup_cons A Gamma i : forall a, @lookup_lt A (a :: Gamma) (fsu i) = lookup_lt Gamma i.
+  destruct i as [i Hi]; simpl; intros; apply lookup_irrel; reflexivity. Qed.
+
+Hint Rewrite lookup_cons.
+
+Theorem lookup_scoped (Gamma : con) (Hg : scoped_con Gamma) :
+  forall i (Hi : i < length Gamma), scoped_at (length Gamma - S i) (lookup_lt Gamma (exist _ i Hi)).
+  Hint Rewrite <- minus_n_O.
+  induction Hg; try (inversion Hi; fail); intros.
+  - destruct i; simpl in *; [rewrite <- minus_n_O; auto|apply IHHg].
 Qed.
 
-Definition prop_and {A B C D} : {A} + {B} -> {C} + {D} -> {A /\ C} + {B \/ D}. auto. Qed.
-Infix "&p&" := prop_and (at level 500, left associativity).
+Lemma lookup_lt_con A (Gamma : list A) : forall i, lookup_con Gamma (`i) = inleft (lookup_lt Gamma i).
+  induction Gamma; intro i; simpl in i; destruct i as [i Hi]; [omega|]; destruct i; [reflexivity|].
+  assert (H: i < length Gamma) by omega; specialize (IHGamma (exist _ i H)); simpl in *; 
+  rewrite IHGamma; f_equal; apply lookup_irrel; auto.
+Qed.  
+  
+Hint Resolve lookup_scoped.
 
-Local Hint Extern 1 => inversion 1; subst.
-Local Hint Extern 1 => econstructor; eassumption.
+Program Definition lookup_wk (Gamma : con) (i : {x | x < length Gamma}) := wk_deep (S i) 0 (lookup_lt Gamma i).
 
-Ltac assert_uqs :=
-  repeat match goal with
-           | [H1 : ?Gamma ⊢ ?e ∈ ?T1 , H2 : ?Gamma ⊢ ?e ∈ ?T2 |- _]
-             => assert (T1 = T2) by (eapply typ_uq; eassumption); subst; clear H2
-         end.
+Program Definition lookup_wk_scoped_subset (Gamma : {gamma | scoped_con gamma}) i : scoped_at (length Gamma) (lookup_wk Gamma i) :=
+  wk_scoped (lookup_lt Gamma i) (length Gamma - S i) _ (S i) 0.
 
-Ltac assert_uqs_inv :=
-  repeat match goal with
-           | [H1 : ?Gamma ⊢ ?e ∈ ?T1 , H2 : ?Gamma ⊢ ?e ∈ ?T2 |- _]
-             => assert (H:T1 = T2) by (eapply typ_uq; eassumption); inversion H; subst; clear H2
-         end.
+(* split for nicer proof terms *)
+Lemma lookup_wk_scoped (Gamma : con) (p : scoped_con Gamma) : forall i, scoped_at (length Gamma) (lookup_wk Gamma i).
+  apply (lookup_wk_scoped_subset (exist _ Gamma p)). Qed.
 
-Local Hint Extern 1 => assert_uqs.
+Hint Resolve lookup_wk_scoped.
 
-Theorem ty_check e : forall Gamma, {T | has_type Gamma e T} + {forall T, ~has_type Gamma e T}.
-  induction e; intros;
-  (* make var do the right thing *)
-  try (destruct (lt_dec ix (length Gamma)) as [Hg|nHg];
-       [left; exists (lookup_wk Gamma (exist _ ix Hg)); auto
-       |right; inversion 1; subst; contradiction]);
-  (* trivial cases *)
-  try (left; repeat econstructor; eassumption; fail); try (right; inversion 1; assert_uqs; congruence; fail);
-  (* pi, lam, sigma, wt *)
-  try (destruct (IHe1 Gamma) as [T1 | nT1]; destruct (IHe2 (Gamma ▻ e1)) as [T2 | nT2];
-       try (right; inversion 1; eapply nT1 || eapply nT2; eassumption);
-       destruct T1 as [T1 Ht1]; try destruct T2 as [T2 Ht2];
-       destruct T1; try (right; inversion 1; subst; assert_uqs; congruence; fail);
-       destruct T2; try (right; inversion 1; subst; assert_uqs; congruence; fail);
-       left; repeat econstructor; eassumption).
-  (* app *)
-  - destruct (IHe1 Gamma) as [T1 | nT1]; destruct (IHe2 Gamma) as [T2 | nT2];
-    try destruct T1 as [T1 Ht1]; try destruct T2 as [T2 Ht2];
-    try (right; inversion 1; eapply nT1 || eapply nT2; eassumption).
-    + destruct T1; try (right; inversion 1; subst; assert_uqs; congruence; fail).
-      destruct (T2 == T1_1); [left|right; inversion 1; assert_uqs; congruence]; subst; repeat econstructor; eassumption.
-  (* smk *)
-  - destruct (IHe2 Gamma) as [T2 | nT2]; destruct (IHe3 Gamma) as [T3 | nT3];
-    try (right; inversion 1; eapply nT2 || eapply nT3; eassumption);
-    destruct T2 as [T2 Ht2]; destruct T3 as [T3 Ht3].
-    destruct (T3 == subst_deep e2 0 e1); subst;
-    [left; repeat econstructor; eassumption|right; inversion 1; subst; assert_uqs; congruence].
-  (* srec *)
-  - destruct (IHe3 Gamma) as [T3 | nT3]; [|right; inversion 1; eapply nT3; eassumption].
-    destruct T3 as [T3 Ht3]; destruct T3; try (right; inversion 1; assert_uqs; congruence).
-    destruct (IHe2 (Gamma ▻ T3_1 ▻ T3_2)) as [T2|nT2]; [destruct T2 as [T2 Ht2]|].
-    + destruct (T2 == subst_deep (smk T3_2 (&1) (&0)) 0 (wk_deep 2 1 e1)).
-      * left; subst; repeat econstructor; eassumption.
-      * right; inversion 1; subst; assert_uqs; inversion H0; subst; assert_uqs; congruence.
-    + right; inversion 1; subst; assert_uqs; inversion H0; subst; eapply nT2; eassumption.
-  (* sup *)
-  - destruct (IHe2 Gamma) as [T2|nT2]; [|right; inversion 1; eapply nT2; eassumption].
-    destruct T2 as [T2 Ht2]; destruct (IHe1 (Gamma ▻ T2)) as [T1|nT1]; [|right; inversion 1; assert_uqs; eapply nT1; eassumption].
-    destruct T1 as [T1 Ht1]; destruct T1; try (right; inversion 1; assert_uqs; congruence).
-    destruct (IHe3 (Gamma ▻ subst_deep e2 0 e1)) as [T3|nT3]; [|right; inversion 1; assert_uqs; eapply nT3; eassumption].
-    destruct T3 as [T3 Ht3]; destruct (T3 == wk_at 0 (wt T2 e1)); [|right; inversion 1; assert_uqs;congruence].
-    + left; subst; repeat econstructor; eassumption.
-  (* wrec *)
-  - destruct (IHe3 Gamma) as [T3|nT3]; [|right; inversion 1; eapply nT3; eassumption].
-    destruct T3 as [T3 Ht3].
-    destruct T3; try (right; inversion 1; assert_uqs; congruence).
-    destruct (IHe2 (Gamma ▻ T3_1 ▻ pi T3_2 (wk_deep 2 0 (wt T3_1 T3_2)) ▻ wk_at 1 T3_2)) as [T2|nT2];
-      [|right; inversion 1; assert_uqs; inversion H6; subst; assert_uqs; eapply nT2; eauto].
-    destruct T2 as [T2 Ht2]; destruct (T2 == subst_deep (&1 @ &0) 0 (wk_deep 3 1 e1));
-      [subst; left; repeat econstructor; eassumption
-      |right; inversion 1; subst; assert_uqs; inversion H0; subst; assert_uqs; congruence].
-  (* brec *)
-  - destruct (IHe2 Gamma) as [T2|nT2]; destruct (IHe3 Gamma) as [T3|nT3]; destruct (IHe4 Gamma) as [T4|nT4];
-    try (right; inversion 1; assert_uqs; eapply nT2 || eapply nT3 || eapply nT4; eassumption);
-    destruct T2 as [T2 Ht2]; destruct T3 as [T3 Ht3]; destruct T4 as [T4 Ht4];
-    destruct T4 , (T2 == subst_deep true 0 e1) , (T3 == subst_deep false 0 e1);
-    try (right; inversion 1; assert_uqs; congruence);
-    subst; left; repeat econstructor; eassumption.
-  (* urec *)
-  - destruct (IHe2 Gamma) as [T2|nT2]; destruct (IHe3 Gamma) as [T3|nT3];
-    try (right; inversion 1; assert_uqs; eapply nT2 || eapply nT3; eassumption);
-    destruct T2 as [T2 Ht2]; destruct T3 as [T3 Ht3];
-    destruct T3 , (T2 == subst_deep unit 0 e1); try (right; inversion 1; assert_uqs; congruence);
-    subst; left; repeat econstructor; eassumption.
-  (* exf *)
-  - destruct (IHe1 (Gamma ▻ bot)) as [T1|nT1]; destruct (IHe2 Gamma) as [T2|nT2];
-    try (right; inversion 1; assert_uqs; eapply nT1 || eapply nT2; eassumption);
-    destruct T1 as [T1 Ht1]; destruct T2 as [T2 Ht2];
-    destruct T1; try (right; inversion 1; assert_uqs; congruence);
-    (* separately because case explosion = bad *)
-    destruct T2; try (right; inversion 1; assert_uqs; congruence);
-    subst; left; repeat econstructor; eassumption.
-Defined.
+Infix "▻" := (fun Gamma a => cons a Gamma) (at level 50, left associativity).
+Infix "-->" := (fun a b => pi a (wk_deep 1 0 b)) (at level 20, right associativity).
+
+Reserved Notation "Gamma ⊢ t ∈ T" (at level 85).
+
+Inductive has_type (Gamma: con) : exp -> exp -> Prop :=
+| ty_var : forall i, Gamma ⊢ & (` i) ∈ lookup_wk Gamma i
+
+| ty_set : forall n, Gamma ⊢ typ n ∈ typ (S n)
+(* (* for now, how about no? *)
+| ty_cumulative : forall A n, Gamma ⊢ A ∈ typ n
+                       -> Gamma ⊢ A ∈ typ (S n)
+
+| ty_pi_prop : forall A P n, Gamma ⊢ A ∈ (typ n)
+                      -> Gamma ▻ A ⊢ P ∈ prop
+                      -> Gamma ⊢ pi A P ∈ prop
+*)
+| ty_pi_typ : forall A B n m, Gamma ⊢ A  ∈ typ n
+                       -> Gamma ▻ A ⊢ B ∈ typ m
+                       -> Gamma ⊢ pi A B ∈ typ (max n m)
+
+| ty_sg_typ : forall A B n m, Gamma ⊢ A ∈ typ n
+                       -> Gamma ⊢ B ∈ (pi A (typ m))
+                       -> Gamma ⊢ sigma A B ∈ typ (max n m)
+
+| ty_wt_typ : forall A B n m, Gamma ⊢ A ∈ typ n
+                       -> Gamma ⊢ B ∈ (pi A (typ m))
+                       -> Gamma ⊢ wt A B ∈ typ (max n m)
+
+| ty_bool : Gamma ⊢ bool ∈ typ 0
+| ty_top : Gamma ⊢ top ∈ typ 0
+| ty_bot : Gamma ⊢ bot ∈ typ 0
+
+| ty_lam : forall A n B b, Gamma ⊢ A ∈ typ n
+                    -> Gamma ▻ A ⊢ b ∈ B
+                    -> Gamma ⊢ lam A b ∈ pi A B
+
+| ty_app : forall A B f a, Gamma ⊢ f ∈ pi A B
+                    -> Gamma ⊢ a ∈ A
+                    -> Gamma ⊢ f @ a ∈ B |> a // 0
+
+| ty_smk : forall A B a b, Gamma ⊢ a ∈ A
+                    -> Gamma ⊢ b ∈ B @ a
+                    -> Gamma ⊢ smk B a b ∈ sigma A B
+
+| ty_srec : forall A B C f s, Gamma ⊢ f ∈ pi A (pi (wk_deep 1 0 B @ &0) (C @ (smk (wk_deep 2 0 B) (&1) (&0))))
+                       -> Gamma ⊢ s ∈ sigma A B
+                       -> Gamma ⊢ srec C f s ∈ C @ s
+
+| ty_sup : forall A B n a f, Gamma ⊢ B ∈ pi A (typ n)
+                      -> Gamma ⊢ a ∈ A
+                      -> Gamma ⊢ f ∈ ((B @ a) --> wt A B)
+                      -> Gamma ⊢ sup B a f ∈ wt A B
+
+| ty_wrec : forall C A B f w,
+              Gamma ⊢ f ∈ pi A (pi (wk_deep 1 0 B @ &0 --> wk_deep 1 0 (wt A B))
+                             ((pi (wk_deep 2 0 B @ &1) (wk_deep 3 0 C @ (&1 @ &0)))
+                                --> wk_deep 3 0 C @ sup (wk_deep 3 0 B) (&2) (&1)))
+            -> Gamma ⊢ w ∈ wt A B
+            -> Gamma ⊢ wrec C f w ∈ C @ w
+| ty_true : Gamma ⊢ true ∈ bool
+| ty_false : Gamma ⊢ false ∈ bool
+| ty_brec : forall C t f b, 
+              Gamma ⊢ t ∈ C @ true
+            -> Gamma ⊢ f ∈ C @ false
+            -> Gamma ⊢ b ∈ bool
+            -> Gamma ⊢ brec C t f b ∈ C @ b
+
+| ty_unit : Gamma ⊢ unit ∈ top
+| ty_urec : forall C u t, Gamma ⊢ u ∈ C @ unit
+                   -> Gamma ⊢ t ∈ top
+                   -> Gamma ⊢ urec C u t ∈ C @ t
+
+| ty_exf : forall C n f, Gamma ⊢ C ∈ (bot --> typ n)
+                  -> Gamma ⊢ f ∈ bot
+                  -> Gamma ⊢ exf C f ∈ C @ f
+
+| ty_step_to : forall e t1 t2, t1 ==> t2 -> Gamma ⊢ e ∈ t1 -> Gamma ⊢ e ∈ t2
+| ty_step_from : forall e t1 t2, t1 ==> t2 -> Gamma ⊢ e ∈ t2 -> Gamma ⊢ e ∈ t1
+where "Gamma ⊢ t ∈ T" := (has_type Gamma t T).
+
+Hint Constructors has_type.
+
+Notation "⟦ xs ⟧" := (length xs).
+
+Require Import DeBrujin.
+
+Hint Rewrite List.app_length.
+
+Lemma lookup_plus_option A : forall (Delta Gamma : list A) i, forget_prop (lookup_con Gamma i) = forget_prop (lookup_con (Delta ++ Gamma) (⟦Delta⟧ + i)).
+  induction Delta; intros; auto.
+  - rewrite IHDelta; simpl; destruct (lookup_con (Delta ++ Gamma) (⟦Delta⟧ + i)); auto. 
+Qed.
+
+Definition wk_ix n d i : nat := if le_dec d i then n + i else i.
+
+Lemma lookup_plus_option2 A (Gamma Delta delta: list A) : forall i,
+  forget_prop (lookup_con (Gamma ++ Delta) i) = forget_prop (lookup_con (Gamma ++ delta ++ Delta) (wk_ix ⟦delta⟧ ⟦Gamma⟧ i)).
+  intro i. unfold wk_ix. destruct (le_dec ⟦Gamma⟧ i) as [Hle|Hnle].
+  - generalize dependent i; induction Gamma; intros; simpl in *.
+    + apply lookup_plus_option.
+    + destruct i; [omega|rewrite <- plus_n_Sm]. 
+      assert(H: ⟦Gamma⟧ <= i) by omega; specialize (IHGamma i H); clear H.
+      destruct (lookup_con (Gamma ++ Delta) i) , (lookup_con (Gamma ++ delta ++ Delta) (⟦delta⟧ + i)); inversion IHGamma; subst; auto.
+  - generalize dependent i; induction Gamma; intros; simpl in *; [omega|destruct i]; auto.
+    assert(H: ~ ⟦Gamma⟧ <= i) by omega; specialize (IHGamma i H);
+    destruct (lookup_con (Gamma ++ Delta) i) , (lookup_con (Gamma ++ delta ++ Delta) i); inversion IHGamma; subst; auto.      
+Qed.
+    
+Hint Resolve lookup_plus_option lookup_plus_option2.
+Hint Rewrite lookup_plus_option lookup_plus_option2.
+
+Program Definition lookup_plus_ty A (Gamma Delta : list A) := forall i, lookup_lt Gamma i = lookup_lt (Delta ++ Gamma) (⟦Delta⟧ + i).
+Next Obligation. rewrite List.app_length. omega. Qed.
+
+(* this is complicated because chained reasoning that can only come together at the very end *)
+Lemma lookup_plus A (Gamma Delta : list A) : lookup_plus_ty Gamma Delta. 
+  unfold lookup_plus_ty; intro i.
+  assert (H:inleft (lookup_lt Gamma i) = lookup_con Gamma (` i)) by (symmetry; apply lookup_lt_con).
+  apply (f_equal forget_prop) in H; simpl in H.
+  assert (H1: forget_prop (lookup_con Gamma (` i)) = forget_prop (lookup_con (Delta ++ Gamma) (⟦Delta⟧ + ` i))) by apply lookup_plus_option.
+  assert (Hob: ⟦Delta⟧ + `i < ⟦Delta ++ Gamma⟧) by (rewrite  List.app_length; destruct i; simpl; omega).
+  assert (H2: lookup_con (Delta ++ Gamma) (⟦Delta⟧ + `i) = inleft (lookup_lt (Delta ++ Gamma) (exist _ (⟦Delta⟧ + ` i) Hob))) by
+    apply lookup_lt_con with (i := exist _ (⟦Delta⟧ + ` i) Hob).
+  apply (f_equal forget_prop) in H2; simpl in H2.
+  assert (H3: Some (lookup_lt Gamma i) = Some (lookup_lt (Delta ++ Gamma) (exist _ (⟦Delta⟧ + `i) Hob))) by congruence.
+  inversion H3. rewrite H4. apply lookup_irrel. auto.
+Qed.
+
+Program Definition wk_ix_lt A delta Gamma {Delta:list A} (ix: {i | i < ⟦Gamma ++ Delta⟧}) : {i | i < ⟦Gamma ++ delta ++ Delta⟧} := wk_ix ⟦delta⟧ ⟦Gamma⟧ ix.
+Obligation 1. repeat rewrite List.app_length in *; unfold wk_ix; destr_choices; omega. Qed.
+
+Lemma lookup_plus2 A (Gamma Delta delta : list A) : forall i, lookup_lt (Gamma ++ Delta) i = lookup_lt (Gamma ++ delta ++ Delta) (wk_ix_lt delta Gamma i).
+  unfold wk_ix_lt; intro i.
+  Local Hint Resolve lookup_lt_con.
+  assert (H1: inleft (lookup_lt (Gamma ++ Delta) i) = lookup_con (Gamma ++ Delta) (` i)) by auto.
+  assert (H2: forget_prop (lookup_con (Gamma ++ Delta) (` i)) = forget_prop (lookup_con (Gamma ++ delta ++ Delta) (wk_ix ⟦delta⟧ ⟦Gamma⟧ (`i)))) by auto.
+  assert (Hob: wk_ix ⟦delta⟧ ⟦Gamma⟧ (` i) < ⟦Gamma++delta++Delta⟧)
+   by (clear H1; destruct i; simpl in *; repeat rewrite List.app_length in *; unfold wk_ix; destr_choices; omega).
+  assert (H3: lookup_con (Gamma ++ delta ++ Delta) (wk_ix ⟦delta⟧ ⟦Gamma⟧ (`i)) = inleft (lookup_lt (Gamma ++ delta ++ Delta) (exist _ (wk_ix ⟦delta⟧ ⟦Gamma⟧ (`i)) Hob)))
+   by apply lookup_lt_con with (i := exist _ (wk_ix ⟦delta⟧ ⟦Gamma⟧ (`i)) Hob).
+  apply (f_equal forget_prop) in H1; apply (f_equal forget_prop) in H3; simpl in *.
+  assert (H:lookup_lt (Gamma ++ Delta) i = lookup_lt (Gamma ++ delta ++ Delta) (exist _ (wk_ix ⟦delta⟧ ⟦Gamma⟧ (`i)) Hob)) by congruence.
+  rewrite H; apply lookup_irrel; auto.
+Qed.
+
+Hint Resolve lookup_plus lookup_plus2.
+Hint Rewrite lookup_plus lookup_plus2.
+
+Lemma wk_ix_deep : forall n d i, wk_deep n d (&i) = &(wk_ix n d i).
+  unfold wk_deep,wk_var,wk_ix; intros; destr_choices; f_equal; omega. Qed.
+
+Lemma wk_ix_lt_eq A : forall Gamma delta Delta i, ` (@wk_ix_lt A delta Gamma Delta i) = wk_ix ⟦delta⟧ ⟦Gamma⟧ (` i).
+  reflexivity. Qed.
+
+Lemma wk_typed e : forall T Gamma Delta, Gamma ++ Delta ⊢ e ∈ T -> forall delta, Gamma ++ delta ++ Delta ⊢ wk_deep ⟦delta⟧ ⟦Gamma⟧ e ∈ wk_deep ⟦delta⟧ ⟦Gamma⟧ T.
+(* (* yuck - we'll just admit this for now *)
+  induction e; inversion 1; subst; intros.
+  - rewrite wk_ix_deep. unfold wk_ix. destruct (le_dec ⟦Gamma⟧ (`i)) as [Hle|Hnle].
+    + unfold lookup_wk in *. rewrite lookup_plus2 with (delta := delta) in *. unfold wk_ix_lt; unfold wk_ix; simpl.
+      assert (H0: ⟦delta⟧ + `i < ⟦Gamma ++ delta ++ Delta ⟧) by (clear H; destruct i; simpl in *; repeat rewrite List.app_length in *; omega).
+      erewrite lookup_irrel; [|instantiate (j := exist _ (⟦delta⟧+(`i)) H0); simpl; destr_choices; omega].
+      rewrite wk_deep_wk; [|omega]. rewrite <- plus_n_Sm.
+      destruct i as [i Hi]; simpl in *.
+      replace (wk_deep (S (⟦ delta ⟧ + i)) 0
+       (lookup_lt (Gamma ++ delta ++ Delta)
+          (exist (fun x : nat => x < ⟦ Gamma ++ delta ++ Delta ⟧)
+             (⟦ delta ⟧ + i) H0))) with (lookup_wk (Gamma ++ delta ++ Delta) (exist _ (⟦delta⟧+i) H0)) by auto. 
+      replace (& (⟦ delta ⟧ + i)) with (& (` (exist (fun i => i < ⟦Gamma ++ delta ++ Delta⟧) (⟦delta⟧+i) H0))) by auto.
+      apply ty_var.
+    + *) Admitted.
+
+Inductive wf_con : con -> Prop :=
+| wf_nil : wf_con nil
+| wf_cons : forall Gamma A n, wf_con Gamma -> Gamma ⊢ A ∈ (typ n) -> wf_con (Gamma ▻ A).
+
+Hint Constructors wf_con.
+
+Lemma typ_conv : forall Gamma e t1 t2, t1 ===> t2 -> Gamma ⊢ e ∈ t1 <-> Gamma ⊢ e ∈ t2.
+    induction 1; split; intros; auto.
+    - apply IHclos_refl_trans_1n; eauto.
+    - eapply ty_step_from; [eassumption|]. eapply IHclos_refl_trans_1n; auto.
+Qed.
+
+Lemma ty_var_congr Gamma i T : Gamma ⊢ & (` i) ∈ T -> exists T', lookup_wk Gamma i ===> T' /\ T ===> T'.
+  remember (& (` i)) as i'; induction 1; inversion Heqi'; subst.
+  - unfold lookup_wk; rewrite H0; erewrite lookup_irrel; eauto.
+  - destruct (IHhas_type i eq_refl) as [t1' Ht]; destruct Ht;
+    assert (exists t2', t2 ===> t2' /\ t1' ===> t2') by (apply step_confluent with (e1 := t1); eauto);
+    destr_logic; eexists; split; [eapply rtc_rtc|]; eassumption.
+  - destruct (IHhas_type i eq_refl) as [t1' Ht]; destruct Ht; eauto.
+Qed.
+
+Lemma ty_typ_congr Gamma n T : Gamma ⊢ typ n ∈ T -> T ===> typ (S n).
+  remember (typ n) as tn; induction 1; inversion Heqtn; subst; auto; specialize (IHhas_type eq_refl); eauto.
+  - assert (exists t2', t2 ===> t2' /\ typ (S n) ===> t2') by (apply step_confluent with (e1 := t1); eauto).
+    destruct H2 as [t2' Ht2']; destruct Ht2' as [Ht2' Htyp]; destruct Htyp as [|y z Htyp Ht']; eauto; inversion Htyp.
+Qed.
+
+Lemma ty_pi_congr Gamma A B T : Gamma ⊢ pi A B ∈ T -> exists n m, (Gamma ⊢ A ∈ typ n) /\ (Gamma ▻ A ⊢ B ∈ typ m) /\ T ===> typ (max n m).
+  remember (pi A B) as pab; induction 1; inversion Heqpab; subst; eauto; 
+  destruct (IHhas_type eq_refl) as [n Hn]; destruct Hn as [m Hnm]; destruct Hnm as [Ha Hbt]; destruct Hbt as [Hb Ht];
+  exists n; exists m; repeat split; eauto.
+  - assert (exists t2', t2 ===> t2' /\ typ (max n m) ===> t2') by (apply step_confluent with (e1 := t1); eauto).
+    destruct H2 as [t2' Ht2']; destruct Ht2' as [Ht2' Htyp]; destruct Htyp as [|y z Htyp Ht']; eauto; inversion Htyp.
+Qed.
+
+Lemma ty_sg_congr Gamma A B T : Gamma ⊢ sigma A B ∈ T -> exists n m, (Gamma ⊢ A ∈ typ n) /\ (Gamma ⊢ B ∈ pi A (typ m)) /\ T ===> typ (max n m).
+  remember (sigma A B) as pab; induction 1; inversion Heqpab; subst; eauto; 
+  destruct (IHhas_type eq_refl) as [n Hn]; destruct Hn as [m Hnm]; destruct Hnm as [Ha Hbt]; destruct Hbt as [Hb Ht];
+  exists n; exists m; repeat split; eauto.
+  - assert (exists t2', t2 ===> t2' /\ typ (max n m) ===> t2') by (apply step_confluent with (e1 := t1); eauto).
+    destruct H2 as [t2' Ht2']; destruct Ht2' as [Ht2' Htyp]; destruct Htyp as [|y z Htyp Ht']; eauto; inversion Htyp.
+Qed.
+
+Lemma ty_wt_congr Gamma A B T : Gamma ⊢ wt A B ∈ T -> exists n m, (Gamma ⊢ A ∈ typ n) /\ (Gamma ⊢ B ∈ pi A (typ m)) /\ T ===> typ (max n m).
+  remember (wt A B) as pab; induction 1; inversion Heqpab; subst; eauto; 
+  destruct (IHhas_type eq_refl) as [n Hn]; destruct Hn as [m Hnm]; destruct Hnm as [Ha Hbt]; destruct Hbt as [Hb Ht];
+  exists n; exists m; repeat split; eauto.
+  - assert (exists t2', t2 ===> t2' /\ typ (max n m) ===> t2') by (apply step_confluent with (e1 := t1); eauto).
+    destruct H2 as [t2' Ht2']; destruct Ht2' as [Ht2' Htyp]; destruct Htyp as [|y z Htyp Ht']; eauto; inversion Htyp.
+Qed.
+
+Lemma ty_bool_congr Gamma T : Gamma ⊢ bool ∈ T -> T ===> typ 0.
+  remember bool as b; induction 1; inversion Heqb; subst; eauto; specialize (IHhas_type eq_refl).
+  - assert (exists t2', t2 ===> t2' /\ typ 0 ===> t2') by (apply step_confluent with (e1 := t1); eauto).
+    destruct H2 as [t2' Ht2']; destruct Ht2' as [Ht2' Htyp]; destruct Htyp as [|y z Htyp Ht']; eauto; inversion Htyp.
+Qed.  
+
+Lemma ty_top_congr Gamma T : Gamma ⊢ top ∈ T -> T ===> typ 0.
+  remember top as b; induction 1; inversion Heqb; subst; eauto; specialize (IHhas_type eq_refl).
+  - assert (exists t2', t2 ===> t2' /\ typ 0 ===> t2') by (apply step_confluent with (e1 := t1); eauto).
+    destruct H2 as [t2' Ht2']; destruct Ht2' as [Ht2' Htyp]; destruct Htyp as [|y z Htyp Ht']; eauto; inversion Htyp.
+Qed.  
+
+Lemma ty_bot_congr Gamma T : Gamma ⊢ bot ∈ T -> T ===> typ 0.
+  remember bot as b; induction 1; inversion Heqb; subst; eauto; specialize (IHhas_type eq_refl).
+  - assert (exists t2', t2 ===> t2' /\ typ 0 ===> t2') by (apply step_confluent with (e1 := t1); eauto).
+    destruct H2 as [t2' Ht2']; destruct Ht2' as [Ht2' Htyp]; destruct Htyp as [|y z Htyp Ht']; eauto; inversion Htyp.
+Qed.
+
+Lemma ty_true_congr Gamma T : Gamma ⊢ true ∈ T -> T ===> bool.
+  remember true as b; induction 1; inversion Heqb; subst; eauto; specialize (IHhas_type eq_refl).
+  - assert (exists t2', t2 ===> t2' /\ bool ===> t2') by (apply step_confluent with (e1 := t1); eauto).
+    destruct H2 as [t2' Ht2']; destruct Ht2' as [Ht2' Htyp]; destruct Htyp as [|y z Htyp Ht']; eauto; inversion Htyp.
+Qed.
+
+Lemma ty_false_congr Gamma T : Gamma ⊢ false ∈ T -> T ===> bool.
+  remember false as b; induction 1; inversion Heqb; subst; eauto; specialize (IHhas_type eq_refl).
+  - assert (exists t2', t2 ===> t2' /\ bool ===> t2') by (apply step_confluent with (e1 := t1); eauto).
+    destruct H2 as [t2' Ht2']; destruct Ht2' as [Ht2' Htyp]; destruct Htyp as [|y z Htyp Ht']; eauto; inversion Htyp.
+Qed.
+
+Lemma ty_unit_congr Gamma T : Gamma ⊢ unit ∈ T -> T ===> top.
+  remember unit as b; induction 1; inversion Heqb; subst; eauto; specialize (IHhas_type eq_refl).
+  - assert (exists t2', t2 ===> t2' /\ top ===> t2') by (apply step_confluent with (e1 := t1); eauto).
+    destruct H2 as [t2' Ht2']; destruct Ht2' as [Ht2' Htyp]; destruct Htyp as [|y z Htyp Ht']; eauto; inversion Htyp.
+Qed.
+
+Lemma wk_step_congr e1 e2 n d : e1 ==> e2 -> wk_deep n d e1 ===> wk_deep n d e2. auto. Qed.
+Lemma wk_eval_congr e1 e2 n d : e1 ===> e2 -> wk_deep n d e1 ===> wk_deep n d e2. 
+  induction 1; eauto; eapply rtc_rtc; [eapply wk_step_congr|]; eassumption. Qed.
+
+Hint Resolve wk_eval_congr.
+
+Lemma con_var_congr Gamma T i t1 t2 (Ht : t1 ===> t2) : t1 :: Gamma ⊢ &i ∈ T <-> t2 :: Gamma ⊢ &i ∈ T.
+  remember (&i) as ix; split; intro Hi.
+  - generalize dependent t2. remember (t1 :: Gamma) as gamma. induction Hi; inversion Heqgamma; inversion Heqix; subst; intros.
+    + destruct i0 as [i Hi]; simpl in *.
+      destruct i; unfold lookup_wk; simpl.
+      * eapply typ_conv; [eapply wk_eval_congr;eassumption|].
+        replace (&0) with (&(` (exist (fun n => n < S (length Gamma)) 0 Hi))) by auto;
+        replace (wk_deep 1 0 t2) with (lookup_wk (t2 :: Gamma) (exist _ 0 Hi)) by auto;
+        constructor.
+      * replace (&(S i)) with (& (` (exist (fun n => n < ⟦t2 :: Gamma⟧) (S i) Hi))) by auto.
+        rewrite <- lookup_cons with (a := t2). unfold fsu. erewrite lookup_irrel. apply ty_var. auto.
+    + specialize (IHHi eq_refl eq_refl).
+Admitted.
+
+Lemma con_cons_congr1 e : forall t1 t2, t1 ===> t2 -> forall Gamma T, (t1 :: Gamma) ⊢ e ∈ T <-> (t2 :: Gamma) ⊢ e ∈ T.
+  induction e; intros; eauto.
+  - split; inversion 1; subst; auto.
+    + destruct i as [i Hi]; induction i.
+Admitted.
+
+Hint Resolve con_cons_congr1.
+Hint Rewrite con_cons_congr1.
+
+Lemma ty_lam_congr Gamma e1 e2 T : Gamma ⊢ lam e1 e2 ∈ T -> exists A B, T ===> pi A B /\ (Gamma ▻ A ⊢ e2 ∈ B) /\ e1 ===> A.
+  intro Ht; remember (lam e1 e2) as lae; induction Ht; inversion Heqlae; subst; [repeat eexists;eauto| |];
+  destruct (IHHt eq_refl) as [A Hb]; destruct Hb as [B Hab]; destruct Hab as [He2 Het];
+  destruct Het as [He1 HT]; clear IHHt;
+  assert (Ht3: exists t3, t2 ===> t3 /\ pi A B ===> t3) by (eapply step_confluent; [|eassumption]; eauto);
+  destruct Ht3 as [t3 Ht3]; destruct Ht3 as [H23 Hpi]; destr_logic; [|repeat eexists; eauto].
+  - extend (eval_pi_pi Hpi); destr_logic; subst; destr_logic.
+    repeat eexists; [eassumption| |].
+    + erewrite <- con_cons_congr1; [|eassumption];erewrite <- typ_conv; eassumption.
+    + eapply rtc_rtc; eassumption.
+Qed.
+
+Lemma ty_sup_congr Gamma e1 e2 e3 T : 
+  Gamma ⊢ sup e1 e2 e3 ∈ T -> exists A B, T ===> wt A B /\ e1 ===> B /\ (Gamma ⊢ e2 ∈ A) /\ (Gamma ⊢ e3 ∈ (B @ e2 --> wt A B)).
+  intro Ht; remember (sup e1 e2 e3) as sae; induction Ht; inversion Heqsae; subst; [repeat eexists;eauto| |];
+  destruct (IHHt eq_refl) as [A Hb]; destruct Hb as [B Hab]; destruct Hab as [Ht1 He]; destruct He as [Heb He3];
+  assert (Ht3: exists t3, t2 ===> t3 /\ wt A B ===> t3) by (eapply step_confluent; [|eassumption]; eauto);
+  destruct Ht3 as [t3 Ht3]; destruct Ht3 as [H23 Hwt];
+  extend (eval_wt_wt Hwt); destr_logic; subst;
+  (repeat eexists;
+   [eassumption || eauto
+   |eapply rtc_rtc; eauto
+   |erewrite <- typ_conv; eauto
+   |erewrite <- typ_conv; [eassumption|apply pi_rtc_cong; [apply app_rtc_cong|]; eauto]]).
+Qed.
+
+Lemma ty_smk_congr Gamma e1 e2 e3 T : 
+  Gamma ⊢ smk e1 e2 e3 ∈ T -> exists A B, T ===> sigma A B /\ e1 ===> B /\ (Gamma ⊢ e2 ∈ A) /\ (Gamma ⊢ e3 ∈ B @ e2).
+  intro Ht; remember (smk e1 e2 e3) as sae; induction Ht; inversion Heqsae; subst; [repeat eexists; eauto| |];
+  destruct (IHHt eq_refl) as [A Hb]; destruct Hb as [B Hab]; destruct Hab as [Ht1 He]; destruct He as [Heb He3];
+  assert (Ht3: exists t3, t2 ===> t3 /\ sigma A B ===> t3) by (eapply step_confluent; [|eassumption]; eauto);
+  destruct Ht3 as [t3 Ht3]; destruct Ht3 as [H23 Hsg];
+  extend (eval_sg_sg Hsg); destr_logic; subst;
+  (repeat eexists;
+   [eassumption || eauto
+   |eapply rtc_rtc; eauto
+   |erewrite <- typ_conv; eauto
+   |erewrite <- typ_conv; [eassumption|apply app_rtc_cong]; eauto]).
+Qed.
+
+(* Lemma preservation : forall e1 e2, e1 ~> e2 -> forall Gamma t, Gamma ⊢ e1 ∈ t -> Gamma ⊢ e2 ∈ t. *)
+
+Hint Resolve ty_var_congr ty_typ_congr.
+Hint Resolve ty_pi_congr ty_sg_congr ty_wt_congr.
+Hint Resolve ty_lam_congr ty_sup_congr ty_smk_congr.
+Hint Resolve ty_top_congr ty_bot_congr ty_bool_congr.
+Hint Resolve ty_true_congr ty_false_congr ty_unit_congr.
+
+Lemma typ_confluent : forall Gamma e t1, Gamma ⊢ e ∈ t1 -> forall t2, Gamma ⊢ e ∈ t2 -> exists t3, t1 ===> t3 /\ t2 ===> t3.
+  induction 1; intros t' Ht'; eauto.
+  - apply ty_pi_congr in Ht'; destr_logic; try_hyps; destr_logic; clear_funs;
+    repeat match goal with [H: pi _ _ ===> _|-_] => extend (eval_pi_pi H) end; destr_logic; subst;
+    repeat match goal with [H: typ _ ===> _|-_] => inversion H as [|y z H']; clear H; [subst|inversion H'] end;
+    repeat match goal with [H: ?e1 = ?e2 |- _] => tryif (atomic e1; atomic e2) then fail else inversion H; subst; clear H end;
+    eauto.
+  - apply ty_sg_congr in Ht'; destr_logic; try_hyps; destr_logic; clear_funs;
+    repeat match goal with [H: pi _ _ ===> _|-_] => extend (eval_pi_pi H) end; destr_logic; subst;
+    repeat match goal with [H: typ _ ===> _|-_] => inversion H as [|y z H']; clear H; [subst|inversion H'] end;
+    repeat match goal with [H: ?e1 = ?e2 |- _] => tryif (atomic e1; atomic e2) then fail else inversion H; subst; clear H end;
+    eauto.
+  - apply ty_wt_congr in Ht'; destr_logic; try_hyps; destr_logic; clear_funs;
+    repeat match goal with [H: pi _ _ ===> _|-_] => extend (eval_pi_pi H) end; destr_logic; subst;
+    repeat match goal with [H: typ _ ===> _|-_] => inversion H as [|y z H']; clear H; [subst|inversion H'] end;
+    repeat match goal with [H: ?e1 = ?e2 |- _] => tryif (atomic e1; atomic e2) then fail else inversion H; subst; clear H end;
+    eauto.
+  - apply ty_lam_congr in Ht'. shelve (* doesn't quite work - needs the correct context shift *).
+  (* not dealing with more cases for now *)
+Admitted.
+
+Theorem preservation : forall Gamma e1 e2 T, e1 ===> e2 -> Gamma ⊢ e1 ∈ T <-> Gamma ⊢ e2 ∈ T.
+Admitted.
+
+(* this induction principle won't quite work - should be a fixpoint, but not yet sure what the measure should be *)
+(* => would be wrong since there are nonterminating (but untyped) programs... hmmm... *)
+
+Theorem ty_normal : forall Gamma e T, Gamma ⊢ e ∈ T -> exists e', e ===> e' /\ is_normal e'.
+  induction 1; auto; try (eexists; split; eauto; inversion 1; fail).
+  - destr_logic; exists (pi x0 x); split; [apply pi_rtc_cong|inversion 1; subst]; unfold is_normal in *; try_hyps; eauto.
+  - destr_logic; exists (sigma x0 x); split; [apply sg_rtc_cong|inversion 1; subst]; unfold is_normal in *; try_hyps; eauto.
+  - destr_logic; exists (wt x0 x); split; [apply wt_rtc_cong|inversion 1; subst]; unfold is_normal in *; try_hyps; eauto.
+  - destr_logic; exists (lam x0 x); split; [apply lam_rtc_cong|inversion 1; subst]; unfold is_normal in *; try_hyps; eauto.
+Admitted.
+
+Theorem ty_check : forall Gamma e, {T | Gamma ⊢ e ∈ T} + {forall T, ~ (Gamma ⊢ e ∈ T)}.
+Admitted.
