coq-in-coq/Unscoped.v
@@ -10,16 +10,19 @@ Inductive exp : Set :=
 
 | sigma : forall(A B : exp), exp
 | smk : forall(B a b : exp), exp
+(* Γ ⊢ p ∈ (a : A) (b : B a) -> C (smk B a b) , Γ ⊢ s ∈ σ A B ⊃ Γ ⊢ srec C p s ∈ C s *)
 | srec : forall(C p s : exp), exp
 
 | wt : forall(A B : exp), exp
+(* Γ ⊢ a ∈ A , Γ ⊢ f ∈ B a -> wt A B ⊃ Γ ⊢ sup B a f ∈ wt A B *)
 | sup : forall(B a f : exp), exp
+(* Γ ⊢ s ∈ (a : A) (f : B a -> wt A B) (f' : (b : B a) -> C (f b)) , Γ ⊢ w ∈ wt A B ⊃ Γ ⊢ wrec C s w ∈ C w *)
 | wrec : forall(C s w : exp), exp
 
 | bool : exp
 | true : exp
 | false : exp
-| brc : forall(C t f b : exp), exp
+| brec : forall(C t f b : exp), exp
 
 | top : exp
 | unit : exp
@@ -28,8 +31,6 @@ Inductive exp : Set :=
 | bot : exp
 | exf : forall(C f : exp), exp.
 
-Hint Resolve Nat.eq_dec.
-
 Definition exp_size (e : exp) : nat.
   induction e;
   repeat match goal with
@@ -37,53 +38,10 @@ Definition exp_size (e : exp) : nat.
          end; apply 0. Defined.
  (* I think this definition is pretty cool :) *)
 
-Definition exp_eq_dec (e1 e2 : exp) : {e1 = e2} + {e1 <> e2}.
-  decide equality. Qed.
-
-Notation "a # b" := (smk _ a b) (at level 100, right associativity).
-Infix "@" := app (at level 500, left associativity).
-Notation "&" := var.
-
-Inductive scoped_at (n : nat) : exp -> Prop :=
-| scope_var : forall i, i < n -> scoped_at n (& i)
-
-| scope_typ : forall m, scoped_at n (typ m)
-
-| scope_pi : forall a b, scoped_at n a -> scoped_at (S n) b -> scoped_at n (pi a b)
-| scope_lam : forall A b, scoped_at n A -> scoped_at (S n) b -> scoped_at n (lam A b)
-| scope_app : forall f x, scoped_at n f -> scoped_at n x -> scoped_at n (f @ x)
-
-| scope_sigma : forall a b, scoped_at n a -> scoped_at (S n) b -> scoped_at n (sigma a b)
-| scope_smk : forall B a b, scoped_at (S n) B -> scoped_at n a -> scoped_at n b -> scoped_at n (smk B a b)
-| scope_srec : forall c p s, scoped_at (S n) c -> scoped_at (2 + n) p -> scoped_at n s
-                       -> scoped_at n (srec c p s)
-
-| scope_wt : forall a b, scoped_at n a -> scoped_at (S n) b -> scoped_at n (wt a b)
-| scope_sup : forall B a f, scoped_at (S n) B -> scoped_at n a -> scoped_at (S n) f -> scoped_at n (sup B a f)
-| scope_wrec : forall c s w, scoped_at (S n) c -> scoped_at (3 + n) s -> scoped_at n w
-                       -> scoped_at n (wrec c s w)
-
-| scope_bool : scoped_at n bool
-| scope_true : scoped_at n true
-| scope_false : scoped_at n false
-| scope_brc : forall c t f b, scoped_at (S n) c -> scoped_at n t -> scoped_at n f -> scoped_at n b
-                         -> scoped_at n (brc c t f b)
-
-| scope_top : scoped_at n top
-| scope_unit : scoped_at n unit
-| scope_urec : forall c u t, scoped_at (S n) c -> scoped_at n u -> scoped_at n t
-                       -> scoped_at n (urec c u t)
-
-| scope_bot : scoped_at n bot
-| scope_exf : forall c f, scoped_at (S n) c -> scoped_at n f -> scoped_at n (exf c f).
-
-Hint Resolve lt_dec.
-
-Hint Constructors scoped_at.
-Hint Constructors sumbool.
-
 Ltac destr_sums :=
   repeat match goal with
+           | [ H :  _  + {_} |- _ ] => destruct H
+           | [ H :  _  +  _  |- _ ] => destruct H
            | [ H : {_} + {_} |- _ ] => destruct H
          end.
 
@@ -96,138 +54,69 @@ Ltac Inster_all := repeat
             clear x; specialize (H x')
   end.
 
-Definition scope_check_at (n : nat) (e : exp) : {scoped_at n e} + {~ scoped_at n e}.
-  (* Local Hint Extern 5 => match goal with [H : scoped_at _ _ |- _] => inversion H end. *)
-  generalize dependent n; induction e; intro n;
-  try (destruct (lt_dec ix n); [left|right]; auto; inversion 1; auto);
-  Inster_all; destr_sums; try (left; constructor; eassumption); right; inversion 1; subst; auto.
-Qed.
+Notation "a # b" := (smk _ a b) (at level 20, right associativity).
+Infix "@" := app (at level 15, left associativity).
+Notation "&" := var.
 
-Fixpoint count_free (e : exp) : nat :=
+Definition and_sumor A1 A2 P1 P2 : A1 + {P1} -> A2 + {P2} -> (A1 * A2) + {P1 \/ P2}.
+  repeat (destruct 1; auto). Defined.
+
+Arguments and_sumor {A1} {A2} {P1} {P2} s1 s2.
+Infix "&&t" := and_sumor (at level 500, left associativity).
+
+Definition prop_and {A B C D} : {A} + {B} -> {C} + {D} -> {A /\ C} + {B \/ D}. repeat (destruct 1; auto). Defined.
+Infix "&&" := prop_and.
+
+Local Hint Extern 1 => subst; (reflexivity || congruence).
+
+Ltac destr_logic := repeat match goal with [H: _ /\ _ |- _] => destruct H | [H: _ \/ _ |- _] => destruct H | [H: exists x, _ |- _] => destruct H end.
+
+Definition exp_eq_dec (e1 e2 : exp) : {e1 = e2} + {e1 <> e2}.
+  generalize dependent e2; induction e1; destruct e2;
+  (* off-diagonal cases *)
+  try (right; inversion 1; fail);
+  (* trivial cases *)
+  try (left;reflexivity);
+  (* vars, typs, etc *)
+  match goal with [n1 : nat , n2 : nat |- _] => destruct (Nat.eq_dec n1 n2); [left|right]; eauto | _ => idtac end;
+  Inster_all;
+  (* everything else *)
+  repeat match goal with [H1: {_} + {_} , H2: {_} + {_} |- _] => remember (prop_and H1 H2) as H12; clear HeqH12; clear H1; clear H2 end;
+  destr_sums; destr_logic; 
+  try (left; repeat match goal with [H: _ = _ |- _] => rewrite H; clear H end; reflexivity);
+  try (right; injection 1; intuition).
+Defined.
+
+(* weakening and substitution have the same recursion structure - lets only write it once *)
+Fixpoint vars_op (op : forall(d ix : nat), exp) (d : nat) (e : exp) : exp :=
   match e with
-    | & i => S i
-    | pi a b => max (count_free a) (pred (count_free b))
-    | sigma a b => max (count_free a) (pred (count_free b))
-    | wt a b => max (count_free a) (pred (count_free b))
-
-    | lam A b => max (count_free A) (pred (count_free b))
-    | (f @ x) => max (count_free f) (count_free x)
-
-    | (smk B a b) => max (max (pred (count_free B)) (count_free a)) (count_free b)
-    | srec c p s => max (max (pred (count_free c)) (pred (pred (count_free p)))) (count_free s)
-
-    | sup B a f => max (max (pred (count_free B)) (count_free a)) (pred (count_free f))
-    | wrec c s w => max (max (pred (count_free c)) (pred (pred (pred (count_free s))))) (count_free w)
-
-    | brc c t f b => max (max (max (pred (count_free c)) (count_free t)) (count_free f)) (count_free b)
-    | urec c u t => max (max (pred (count_free c)) (count_free u)) (count_free t)
-    | exf c f => max (pred (count_free c)) (count_free f)
-    
-    | _ => 0
-  end.
-
-Require Import Omega.
-
-Lemma scoped_at_lift (e : exp) n (p : scoped_at n e) : forall m, n <= m -> scoped_at m e.
-  induction p; intros; constructor; try apply IHp; try apply IHp1; try apply IHp2; try apply IHp3; try apply IHp4; omega.
-Qed.
-
-Hint Resolve scoped_at_lift.
-Hint Resolve Nat.le_max_l Nat.le_max_r.
-
-Hint Extern 1 (?n <= max ?n ?m) => apply Nat.le_max_l.
-
-Lemma le_S_pred : forall n, n <= S (pred n). intro; omega. Qed.
-Lemma S_max_pred : forall n m, S (max n m) = max (S n) (S m). induction n; induction m; auto. Qed.
-
-Hint Rewrite S_max_pred.
-
-Ltac SMax := repeat match goal with
-                      | [ |- context[S (max _ _)] ] => rewrite S_max_pred
-                    end.
-
-Lemma max_trans_l : forall d n m, d <= n -> d <= max n m. intros; eapply le_trans; eauto. Qed.
-Lemma max_trans_r : forall d n m, d <= m -> d <= max n m. intros; eapply le_trans; eauto. Qed.
-Hint Resolve max_trans_l max_trans_r.
-Ltac le_max :=
-  match goal with
-    | [|- ?d <= max ?n ?m] => (eapply max_trans_l; try le_max; omega; fail) || (eapply max_trans_r; try le_max; omega; fail)
-  end.
-Theorem scoped_at_count (e : exp) : scoped_at (count_free e) e.
-  Local Hint Resolve le_n_S.
-  Local Hint Resolve le_S_pred.
-  Local Hint Extern 1 => SMax.
-  induction e; intros;
-  try (constructor; simpl in *; omega);
-  try (constructor; simpl; SMax; (eapply scoped_at_lift; [eassumption|le_max])).
-Qed.
-
-Lemma max_le_eq_l : forall n m, n <= m -> max n m = m.
-  induction n; induction m; inversion 1; subst; simpl; eauto.
-  - f_equal; apply IHn; omega.
-Qed.
-
-Lemma max_le_eq_r : forall n m, n <= m -> max m n = m.
-  induction n; induction m; inversion 1; subst; simpl; eauto.
-  - f_equal; apply IHn; omega.
-Qed.
-
-Lemma max_refl : forall n, max n n = n. intros; apply max_le_eq_l; eauto. Qed.
-
-Hint Rewrite max_le_eq_l max_le_eq_r max_refl.
-Hint Resolve max_le_eq_l max_le_eq_r max_refl.
-
-Lemma max_left_right : forall n m, (max n m = n) \/ (max n m = m).
-  intros; destruct (lt_eq_lt_dec n m) as [Hle|Hgt]; [destruct Hle as [Hlt|Heq]|]; subst;
-  [right;apply max_le_eq_l|right;apply max_refl|left;apply max_le_eq_r]; omega. Qed.
-
-Lemma max_le_trans : forall n m d, n <= d -> m <= d -> max n m <= d.
-  intros; destruct (max_left_right n m) as [Hn|Hm]; [rewrite Hn|rewrite Hm]; eauto. Qed.
-
-Hint Resolve max_le_trans.
-
-(* well, at least this was easy *)
-Theorem count_free_least (e : exp) : forall n, scoped_at n e -> count_free e <= n.
-  induction 1; simpl in *; repeat apply max_le_trans; try omega. Qed. 
-
-(* And now for something completely different... *)
-Fixpoint vars_op (op : forall(ix d : nat), exp) (d : nat) (e : exp) : exp :=
-  match e with
-    | & i => op i d
+    | & i => op d i
 
     | pi a b => pi (vars_op op d a) (vars_op op (S d) b)
-    | sigma a b => sigma (vars_op op d a) (vars_op op (S d) b)
-    | wt a b => wt (vars_op op d a) (vars_op op (S d) b)
-
     | lam A b => lam (vars_op op d A) (vars_op op (S d) b)
     | (f @ x) => app (vars_op op d f) (vars_op op d x)
 
-    | (smk B a b) => smk (vars_op op (S d) B) (vars_op op d a) (vars_op op d b)
-    | srec c p s => srec (vars_op op (S d) c) (vars_op op (2 + d) p) (vars_op op d s)
+    | sigma a b => sigma (vars_op op d a) (vars_op op d b)
+    | (smk B a b) => smk (vars_op op d B) (vars_op op d a) (vars_op op d b)
+    | srec c p s => srec (vars_op op d c) (vars_op op d p) (vars_op op d s)
 
-    | sup B a f => sup (vars_op op (S d) B) (vars_op op d a) (vars_op op (S d) f)
-    | wrec c s w => wrec (vars_op op (S d) c) (vars_op op (3 + d) s) (vars_op op d w)
+    | wt a b => wt (vars_op op d a) (vars_op op d b)
+    | sup B a f => sup (vars_op op d B) (vars_op op d a) (vars_op op d f)
+    | wrec c s w => wrec (vars_op op d c) (vars_op op d s) (vars_op op d w)
 
-    | brc c t f b => brc (vars_op op (S d) c) (vars_op op d t) (vars_op op d f) (vars_op op d b)
-    | urec c u t => urec (vars_op op (S d) c) (vars_op op d u) (vars_op op d t)
-    | exf c f => exf (vars_op op (S d) c) (vars_op op d f)
+    | brec c t f b => brec (vars_op op d c) (vars_op op d t) (vars_op op d f) (vars_op op d b)
+    | urec c u t => urec (vars_op op d c) (vars_op op d u) (vars_op op d t)
+    | exf c f => exf (vars_op op d c) (vars_op op d f)
 
     | _ => e
   end.
 
-Definition wk_var (n ix d : nat) : exp := if le_dec d ix then var (n + ix) else var ix.
+Definition wk_var (n d ix : nat) : exp := if le_dec d ix then var (n + ix) else var ix.
 Definition wk_deep (n : nat) : nat -> exp -> exp := vars_op (wk_var n).
 
 Hint Unfold vars_op wk_var wk_deep.
 
-Theorem wk_scoped (e : exp) n (p : scoped_at n e) : forall m d, scoped_at (m + n) (wk_deep m d e).
-  induction p; intros; unfold wk_deep in *; simpl; try constructor; simpl; repeat rewrite plus_n_Sm; auto.
-  - unfold wk_var; simpl; destruct (le_dec d i); constructor; omega.
-Qed.
-
-Hint Resolve wk_scoped.
-
-Definition subst_var (v : exp) (i d : nat) : exp := match lt_eq_lt_dec i d with
+Definition subst_var (v : exp) (d i : nat) : exp := match lt_eq_lt_dec i d with
                                                     | inleft (left _) => var i
                                                     | inleft (right _) => wk_deep d 0 v
                                                     | inright _ => var (pred i)
@@ -238,272 +127,59 @@ Definition subst_deep (v : exp) : nat -> exp -> exp := vars_op (subst_var v).
 Transparent vars_op.
 Transparent subst_deep.
 Transparent subst_var.
-Notation "e [ x / i ]" := (subst_deep x i e) (at level 300).
-
+Notation "x |> v // d" := (subst_deep v d x) (left associativity, at level 40).
 Hint Unfold subst_deep subst_var.
 
-Lemma subst_scoped_pred (e : exp) n (p : scoped_at n e) :
-  forall d v, d < n -> scoped_at (n - S d) v -> scoped_at (pred n) (subst_deep v d e).
-  induction p; intros d v Hd Hv; (destruct n; simpl in *; [exfalso;omega|]);
-  try constructor;
-  (* try applying all the IH's *)
-  try (apply IHp; [omega|auto]); try (apply IHp1; [omega|auto]);
-  try (apply IHp2; [omega|auto]); try (apply IHp3; [omega|auto]); try (apply IHp4; [omega|auto]).
-  (* vars, the always special case *)
-  - unfold subst_deep; unfold subst_var; simpl; destruct (lt_eq_lt_dec i d) as [Hle|Hgt]; [destruct Hle as [Hlt|_]|];
-    [constructor|replace n with (d + (n - d)) by omega; apply wk_scoped|constructor]; [omega|auto|omega].
-Qed.
 
-Theorem subst_scoped (e : exp) n (p : scoped_at (S n) e) :
-  forall d v, d <= n -> scoped_at (n - d) v -> scoped_at n (subst_deep v d e).
-  replace n with (pred (S n)) by omega; intros; apply subst_scoped_pred; auto. Qed.
+Ltac destr_goal_if :=
+  match goal with 
+    | [|- context[if ?c then _ else _]] => destruct c; simpl
+  end.
 
-Hint Resolve subst_scoped.
-
-Theorem subst_0_scoped (e : exp) n (p : scoped_at (S n) e) v : scoped_at n v -> scoped_at n (subst_deep v 0 e).
-  intro H. replace n with (n - 0) in H by omega. apply subst_scoped; auto; omega. Qed.
-
-Definition con := list exp.
-Open Scope list_scope.
-
-Inductive scoped_con : con -> Prop :=
-| scope_nil : scoped_con nil
-| scope_cons : forall Gamma X, scoped_con Gamma -> scoped_at (length Gamma) X -> scoped_con (X :: Gamma).
-
-Hint Constructors scoped_con.
-
-Require Import Coq.Program.Wf.
-
-Lemma unwk_scoped : forall e n m d, d <= m -> scoped_at (n + m) (wk_deep n d e) -> scoped_at m e.
-  induction e; intros n m d Hd He; simpl in *; try (
-  (* dispatch trivial cases *)
-  try (repeat constructor; auto; fail);
-  (* var case takes some special handling *)
-  try (unfold wk_deep in *; unfold wk_var in *; simpl in *; destruct (le_dec d ix));
-  (* invert and split obligations *)
-  inversion He; subst; constructor; simpl in *; repeat rewrite plus_n_Sm in *;
-  (* try all the IH's *)
-  try eapply (IHe1 n); try eapply (IHe2 n); try eapply (IHe3 n); try eapply (IHe4 n);
-  (* finish the job *)
-  try eassumption; omega).
-Qed.
-
-Hint Resolve unwk_scoped.
-
-Lemma unsubst_scoped : forall e v d n, d <= n -> scoped_at (n - d) v -> scoped_at n (subst_deep v d e) -> scoped_at (S n) e.
-  induction e; intros v d n Hd Hv He; unfold subst_deep in *; simpl in *;
-  (* var case always takes some special care *)
-  try (unfold subst_var in *; simpl in *;
-       destruct (lt_eq_lt_dec ix d) as [Hle|Hgt]; [destruct Hle as [Hlt|Heq]|]; inversion He; constructor; omega);
-  (* invert things and split *)
-  inversion He; subst; repeat constructor;
-  (* try all IH's *)
-  try eapply (IHe v); try eapply (IHe1 v); try eapply (IHe2 v); try eapply (IHe3 v); try eapply (IHe4 v);
+Ltac destr_goal_sum :=
   match goal with
-    (* use ordering cases to instantiate d *)
-    | [|- _ <= _] => repeat (try apply Hd; apply le_n_S in Hd)
-    | _ => assumption (* otherwise it'll just be a piece of He *)
- end.
-Qed.
-
-Lemma unsubst_scoped_O : forall e v n, scoped_at n v -> scoped_at n (subst_deep v 0 e) -> scoped_at (S n) e.
-  intros e v n Hv He; apply unsubst_scoped in He; try rewrite <- minus_n_O; try assumption; omega. Qed.
-
-
-Fixpoint lookup_con {A} (Gamma : list A) (i : nat) : A + {i >= length Gamma} :=
-  match Gamma , i with
-    | nil , _ => inright (Peano.le_0_n i)
-    | (X :: Gamma) , 0 => inleft X
-    | (X :: Gamma) , S n => match lookup_con Gamma n with
-                         | inleft T => inleft T
-                         | inright p => inright (le_n_S _ _ p)
-                       end
+    | [|- context[?s]] => match type of s with
+                          | {_} + {_} => destruct s
+                          | _ + {_} => destruct s
+                        end
   end.
 
-Program Fixpoint lookup_lt {A} (Gamma : list A) (i : {x | x < length Gamma}) : A :=
-  match Gamma , i with
-    | nil , _ => False_rect _ _
-    | (x :: xs) , 0   => x
-    | (x :: xs) , S n => lookup_lt xs n
-  end.
+Tactic Notation "destr_choices" := repeat (destr_goal_if || destr_goal_sum; simpl).
 
-Obligation 1. inversion H. Qed.
-Obligation 2. exact (le_S_n _ _ H). Defined.
+Lemma wk_var_fold : forall n, (fun d ix => if le_dec d ix then &(n + ix) else &ix) = wk_var n. reflexivity. Qed.
+Lemma subst_var_fold : forall v, (fun d i => match lt_eq_lt_dec i d with
+                                           | inleft (left _) => &i
+                                           | inleft (right _) => wk_deep d 0 v
+                                           | inright _ => &(pred i)
+                                         end) = subst_var v. reflexivity. Qed.
 
-Lemma lookup_irrel A (Gamma : list A) : forall i p q, lookup_lt Gamma (exist _ i p) = lookup_lt Gamma (exist _ i q).
-  induction Gamma; [simpl;intros;exfalso;omega|]; destruct i; intros; simpl; eauto.
-Qed.
+Ltac fold_wk := repeat match goal with
+                  | [|-context[vars_op (wk_var ?n)]] => replace (vars_op (wk_var n)) with (wk_deep n) by auto
+                  | [|-context[fun d ix => if le_dec d ix then &(?n + ix) else &ix]] => 
+                    replace (fun d ix => if le_dec d ix then &(n + ix) else &ix) with (wk_var n) by auto
+                  | [H:context[vars_op (wk_var ?n)]|-_] => replace (vars_op (wk_var n)) with (wk_deep n) in H by auto
+                  | [H:context[fun d ix => if le_dec d ix then &(?n + ix) else &ix]|-_] => 
+                    replace (fun d ix => if le_dec d ix then &(n + ix) else &ix) with (wk_var n) in H by auto
+                end.
 
-Hint Rewrite lookup_irrel.
+                     (* | [|-context[fun d i => match lt_eq_lt_dec i d with *)
+                     (*                       | inleft (left _) => &i *)
+                     (*                       | inleft (right _) => wk_deep d 0 ?v *)
+                     (*                       | inright _ => &(pred i) *)
+                     (*                     end]] => *)
+                     (*   replace (fun d i => match lt_eq_lt_dec i d with *)
+                     (*                      | inleft (left _) => &i *)
+                     (*                      | inleft (right _) => wk_deep d 0 v *)
+                     (*                      | inright _ => &(pred i) *)
+                     (*                    end) with (subst_var v) by auto *)
 
-Program Definition fsu {n} : {x | x < n} -> {x | x < S n} := S.
+Ltac fold_subst := 
+  repeat rewrite subst_var_fold in *;
+  repeat match goal with
+           | [|-context[vars_op (subst_var ?v)]] => replace (vars_op (subst_var v)) with (subst_deep v) by auto
+           | [H:context[vars_op (subst_var ?v)]|-_] => replace (vars_op (subst_var v)) with (subst_deep v) in H by auto
+         end.
 
-Lemma lookup_cons A Gamma i : forall a, @lookup_lt A (a :: Gamma) (fsu i) = lookup_lt Gamma i.
-  destruct i as [i Hi]; simpl; erewrite lookup_irrel; reflexivity. Qed.
+Tactic Notation "unfold_ops" := unfold wk_deep,subst_deep,wk_var,subst_var in *.
+Tactic Notation "fold_ops" := fold_wk; fold_subst.
 
-Hint Rewrite lookup_cons.
-
-Lemma lookup_lt_con A (Gamma : list A) : forall (i : nat) (Hi : i < length Gamma), lookup_con Gamma i = inleft (lookup_lt Gamma (exist _ i Hi)).
-  induction Gamma; destruct i; try (inversion Hi; fail); auto; intros.
-  - simpl; rewrite IHGamma with (Hi := (le_S_n _ _ Hi)); reflexivity.
-Qed.
-
-Theorem lookup_scoped (Gamma : con) (Hg : scoped_con Gamma) :
-  forall i (Hi : i < length Gamma), scoped_at (length Gamma - S i) (lookup_lt Gamma (exist _ i Hi)).
-  Hint Rewrite <- minus_n_O.
-  induction Hg; try (inversion Hi; fail); intros.
-  - destruct i; simpl in *; [rewrite <- minus_n_O; auto|apply IHHg with (Hi := le_S_n _ _ Hi)].
-Qed.
-
-Hint Resolve lookup_scoped.
-
-Program Definition lookup_wk (Gamma : con) (i : {x | x < length Gamma}) := wk_deep (S i) 0 (lookup_lt Gamma i).
-
-Program Definition lookup_wk_scoped_prog (Gamma : {gamma | scoped_con gamma}) i : scoped_at (length Gamma) (lookup_wk Gamma i) :=
-  wk_scoped (lookup_lt Gamma i) (length Gamma - S i) _ (S i) 0.
-
-Obligation 2. omega. Qed.
-
-(* split for nicer proof terms *)
-Lemma lookup_wk_scoped (Gamma : con) (p : scoped_con Gamma) : forall i, scoped_at (length Gamma) (lookup_wk Gamma i).
-  apply (lookup_wk_scoped_prog (exist _ Gamma p)). Qed.
-
-Hint Resolve lookup_wk_scoped.
-
-Definition wk_n n := wk_deep n 0.
-Definition wk_at n := wk_deep 1 n.
-
-Definition prop := typ 0.
-Definition set := typ 1.
-
-Infix "▻" := (fun Gamma a => cons a Gamma) (at level 50, left associativity).
-Infix "-->" := (fun a b => pi a (wk_at 0 b)) (at level 100, right associativity).
-
-Inductive has_type (Gamma : con) : exp -> exp -> Prop :=
-| ty_var : forall i p, has_type Gamma (var i) (lookup_wk Gamma (exist _ i p))
-
-| ty_set : forall n, has_type Gamma (typ n) (typ (S n))
-(* (* prop and cumulativity are /annoying/ *) 
-| ty_cumulative : forall A n, has_type Gamma A (typ n)
-                       -> has_type Gamma A (typ (S n))
-
-| ty_pi_prop : forall A P n, has_type Gamma A (typ n)
-                      -> has_type (Gamma ▻ A) P prop
-                      -> has_type Gamma (pi A P) prop
-*)
-| ty_pi_typ : forall A B n m, has_type Gamma A (typ n)
-                       -> has_type (Gamma ▻ A) B (typ m)
-                       -> has_type Gamma (pi A B) (typ (max n m))
-
-| ty_sg_typ : forall A B n m, has_type Gamma A (typ n)
-                       -> has_type (Gamma ▻ A) B (typ m)
-                       -> has_type Gamma (sigma A B) (typ (max n m))
-
-| ty_wt_typ : forall A B n m, has_type Gamma A (typ n)
-                       -> has_type (Gamma ▻ A) B (typ m)
-                       -> has_type Gamma (wt A B) (typ (max n m))
-
-| ty_bool : has_type Gamma bool set
-| ty_top : has_type Gamma top prop
-| ty_bot : has_type Gamma bot prop
-
-| ty_lam : forall A n B b, has_type Gamma A (typ n)
-                    -> has_type (Gamma ▻ A) b B
-                    -> has_type Gamma (lam A b) (pi A B)
-
-| ty_app : forall A B f a, has_type Gamma f (pi A B)
-                    -> has_type Gamma a A
-                    -> has_type Gamma (f @ a) (subst_deep a 0 B)
-
-| ty_smk : forall A B a b, has_type Gamma a A
-                    -> has_type Gamma b (subst_deep a 0 B)
-                    -> has_type Gamma (smk B a b) (sigma A B)
-
-| ty_srec : forall A B C f s, has_type (Gamma ▻ A ▻ B) f (subst_deep (smk B (& 1) (& 0)) 0 (wk_deep 2 1 C))
-                      -> has_type Gamma s (sigma A B)
-                      -> has_type Gamma (srec C f s) (subst_deep s 0 C)
-
-| ty_sup : forall A B n a f, has_type Gamma a A
-                      -> has_type (Gamma ▻ A) B (typ n)
-                      -> has_type (Gamma ▻ subst_deep a 0 B) f (wk_at 0 (wt A B))
-                      -> has_type Gamma (sup B a f) (wt A B)
-
-| ty_wrec : forall C A B f w,
-             has_type (Gamma ▻ A ▻ (pi B (wk_deep 2 0 (wt A B))) ▻ wk_at 1 B) f (subst_deep (& 1 @ & 0) 0 (wk_deep 3 1 C))
-           -> has_type Gamma w (wt A B)
-           -> has_type Gamma (wrec C f w) (subst_deep w 0 C)
-
-| ty_true : has_type Gamma true bool
-| ty_false : has_type Gamma false bool
-| ty_brc : forall C t f b, has_type Gamma t (subst_deep true 0 C)
-                    -> has_type Gamma f (subst_deep false 0 C)
-                    -> has_type Gamma b bool
-                    -> has_type Gamma (brc C t f b) (subst_deep b 0 C)
-
-| ty_unit : has_type Gamma unit top
-| ty_urec : forall C u t, has_type Gamma u (subst_deep unit 0 C)
-                   -> has_type Gamma t top
-                   -> has_type Gamma (urec C u t) (subst_deep t 0 C)
-
-| ty_exf : forall C n f, has_type (Gamma ▻ bot) C (typ n)
-                  -> has_type Gamma f bot
-                  -> has_type Gamma (exf C f) (subst_deep f 0 C).
-
-Notation "Gamma ⊢ t ∈ T" := (has_type Gamma t T) (at level 10).
-Hint Constructors has_type.
-
-Inductive wf_con : con -> Prop :=
-| wf_nil : wf_con nil
-| wf_cons : forall Gamma A n, wf_con Gamma -> Gamma ⊢ A ∈ (typ n) -> wf_con (Gamma ▻ A).
-
-Hint Constructors wf_con.
-
-Theorem typed_implies_scoped : forall Gamma t T, scoped_con Gamma -> Gamma ⊢ t ∈ T -> scoped_at (length Gamma) T /\ scoped_at (length Gamma) t.
-Proof with try eassumption.
-  intros Gamma t T Hg.
-  induction 1; auto; simpl in *; try (repeat constructor; auto; fail);
-  try (destruct (IHhas_type Hg) as [IH1 IH2]);
-  try (destruct (IHhas_type1 Hg) as [IH11 IH12]); try (destruct (IHhas_type2 Hg) as [IH21 IH22]);
-  try (destruct (IHhas_type3 Hg) as [IH31 IH32]); try (destruct (IHhas_type4 Hg) as [IH41 IH42]);
-  try (destruct (IHhas_type2 (scope_cons _ _ Hg IH12)) as [IH21 IH22]);
-  try (split; repeat constructor; auto; fail).
-  (* app is weird *)
-  - split; try (constructor; auto).
-    + inversion IH11; subst; apply subst_0_scoped...
-  - split; try (constructor; auto); (eapply unsubst_scoped_O; [|eassumption])...
-  (* recursion principles will take special handling *)
-  - inversion IH21; subst. assert (Hg' : scoped_con (B :: A :: Gamma)) by auto. destruct (IHhas_type1 Hg') as [IH11 IH12].
-    assert (IHC : scoped_at (S(length Gamma)) C).
-      + apply unwk_scoped with (n := 2) (d := 1); [omega|eapply unsubst_scoped_O]; [|eassumption].
-        * constructor; [eapply scoped_at_lift; [eassumption|]; omega| |]; constructor; omega.
-      + split; [eapply subst_0_scoped; auto|constructor]...
-  (* oh, and so will sup *)
-  - destruct (IHhas_type2 (scope_cons _ _ Hg IH11)) as [IH21 IH22].
-    assert (Hg'' : scoped_con (subst_deep a 0 B :: Gamma)).
-      constructor; [|apply subst_0_scoped]...
-    destruct (IHhas_type3 Hg''); split; auto.
-  (* now for the /really/ fun one, wrec *)
-  - inversion IH21; subst.
-    assert (Hg' : scoped_con (wk_at 1 B :: pi B (wk_deep 2 0 (wt A B)) :: A :: Gamma)).
-      constructor; [constructor ;[constructor|]|];
-      [| |simpl; constructor; try assumption;
-          replace (S (S (length Gamma))) with (2 + length Gamma) by omega;
-          apply wk_scoped; constructor
-       | simpl; replace (S (S (length Gamma))) with (1 + S(length Gamma)) by omega; apply wk_scoped]...
-    destruct (IHhas_type1 Hg') as [IH11 IH12].
-    assert (Hc : scoped_at (S (length Gamma)) C). 
-      apply unsubst_scoped_O in IH11; [|constructor;constructor;omega].
-      apply unwk_scoped with (n := 3) (d := 1); [omega|]...
-    split; [apply subst_0_scoped|constructor]...
-  - assert (Hc : scoped_at (S (length Gamma)) C).
-      eapply unsubst_scoped_O; [|eassumption]; auto.
-    split; [apply subst_0_scoped|constructor]...
-  - assert (Hc : scoped_at (S (length Gamma)) C).
-      eapply unsubst_scoped_O; [|eassumption]; auto.
-    split; [apply subst_0_scoped|constructor]...
-  - destruct (IHhas_type1 (scope_cons _ _ Hg (scope_bot _))) as [IH11 IH12].
-    split; [apply subst_0_scoped|constructor]...
-Qed. (* seems like it ought to be possible to automate more of that, but for now I'll just leave it be *)
-
-Theorem wf_implies_scoped : forall Gamma, wf_con Gamma -> scoped_con Gamma.
-  induction 1; constructor; try eapply typed_implies_scoped; eassumption. Qed.
