coq-in-coq/Evaluation.v
@@ -1,0 +1,392 @@
+Set Implicit Arguments.
+Require Import Unscoped.
+Require Import DeBrujin.
+Require Import Omega.
+
+Reserved Notation "a ~> b" (at level 50).
+
+Inductive par_red : exp -> exp -> Prop :=
+| par_ref : forall e, e ~> e
+
+| par_pi : forall e1 e1' e2 e2', e1 ~> e1' -> e2 ~> e2' -> pi e1 e2 ~> pi e1' e2'
+| par_lam : forall e1 e1' e2 e2', e1 ~> e1' -> e2 ~> e2' -> lam e1 e2 ~> lam e1' e2'
+| par_app : forall e1 e1' e2 e2', e1 ~> e1' -> e2 ~> e2' -> (e1 @ e2) ~> (e1' @ e2')
+| par_app_lam : forall e1 e2 e3 e4 e5, e1 ~> lam e2 e3 -> e4 ~> e5 -> e1 @ e4 ~> e3 |> e5 // 0
+
+| par_sg : forall e1 e1' e2 e2', e1 ~> e1' -> e2 ~> e2' -> sigma e1 e2 ~> sigma e1' e2'
+| par_smk : forall e1 e1' e2 e2' e3 e3', e1 ~> e1' -> e2 ~> e2' -> e3 ~> e3' -> smk e1 e2 e3 ~> smk e1' e2' e3'
+| par_srec : forall e1 e1' e2 e2' e3 e3', e1 ~> e1' -> e2 ~> e2' -> e3 ~> e3' -> srec e1 e2 e3 ~> srec e1' e2' e3'
+| par_srec_smk : forall e1 e2 e2' e3 e4 e5 e6, e2 ~> e2' -> e3 ~> smk e4 e5 e6
+                                          -> srec e1 e2 e3 ~> e2' @ e5 @ e6
+
+| par_wt : forall e1 e1' e2 e2', e1 ~> e1' -> e2 ~> e2' -> wt e1 e2 ~> wt e1' e2'
+| par_sup : forall e1 e1' e2 e2' e3 e3', e1 ~> e1' -> e2 ~> e2' -> e3 ~> e3' -> sup e1 e2 e3 ~> sup e1' e2' e3'
+| par_wrec : forall e1 e1' e2 e2' e3 e3', e1 ~> e1' -> e2 ~> e2' -> e3 ~> e3' -> wrec e1 e2 e3 ~> wrec e1' e2' e3'
+| par_wrec_sup : forall e1 e1' e2 e2' e3 e4 e5 e6, e1 ~> e1' -> e2 ~> e2' -> e3 ~> sup e4 e5 e6
+                 -> wrec e1 e2 e3 ~> e2' @ e5 @ (lam (e4 @ e5) (wrec (wk_deep 1 0 e1') (wk_deep 1 0 e2') (wk_deep 1 0 e6 @ &0)))
+
+| par_brec : forall e1 e1' e2 e2' e3 e3' e4 e4', e1 ~> e1' -> e2 ~> e2' -> e3 ~> e3' -> e4 ~> e4' -> brec e1 e2 e3 e4 ~> brec e1' e2' e3' e4'
+| par_brec_true : forall e1 e1' e2 e2' e3 e3' e4, e1 ~> e1' -> e2 ~> e2' -> e3 ~> e3' -> e4 ~> true
+                                             -> brec e1 e2 e3 e4 ~> e2'
+| par_brec_false : forall e1 e1' e2 e2' e3 e3' e4, e1 ~> e1' -> e2 ~> e2' -> e3 ~> e3' -> e4 ~> false
+                                              -> brec e1 e2 e3 e4 ~> e3'
+
+| par_urec : forall e1 e1' e2 e2' e3 e3', e1 ~> e1' -> e2 ~> e2' -> e3 ~> e3' -> urec e1 e2 e3 ~> urec e1' e2' e3'
+| par_urec_unit : forall e1 e1' e2 e2' e3, e1 ~> e1' -> e2 ~> e2' -> e3 ~> unit -> urec e1 e2 e3 ~> e2'
+
+| par_exf : forall e1 e1' e2 e2', e1 ~> e1' -> e2 ~> e2' -> exf e1 e2 ~> exf e1' e2'
+where "a ~> b" := (par_red a b).
+
+Reserved Notation "a ==> b" (at level 50).
+Inductive step : exp -> exp -> Prop :=
+| step_pi1 : forall e1 e1' e2, e1 ==> e1' -> pi e1 e2 ==> pi e1' e2
+| step_pi2 : forall e1 e2 e2', e2 ==> e2' -> pi e1 e2 ==> pi e1 e2'
+| step_lam1 : forall e1 e1' e2, e1 ==> e1' -> lam e1 e2 ==> lam e1' e2
+| step_lam2 : forall e1 e2 e2', e2 ==> e2' -> lam e1 e2 ==> lam e1 e2'
+| step_app1 : forall e1 e1' e2, e1 ==> e1' -> app e1 e2 ==> app e1' e2
+| step_app2 : forall e1 e2 e2', e2 ==> e2' -> app e1 e2 ==> app e1 e2'
+| step_app_lam : forall e1 e2 e3, (lam e1 e2) @ e3 ==> e2 |> e3 // 0
+
+| step_sg1 : forall e1 e1' e2, e1 ==> e1' -> sigma e1 e2 ==> sigma e1' e2
+| step_sg2 : forall e1 e2 e2', e2 ==> e2' -> sigma e1 e2 ==> sigma e1 e2'
+| step_smk1 : forall e1 e1' e2 e3, e1 ==> e1' -> smk e1 e2 e3 ==> smk e1' e2 e3
+| step_smk2 : forall e1 e2 e2' e3, e2 ==> e2' -> smk e1 e2 e3 ==> smk e1 e2' e3
+| step_smk3 : forall e1 e2 e3 e3', e3 ==> e3' -> smk e1 e2 e3 ==> smk e1 e2 e3'
+| step_srec1 : forall e1 e1' e2 e3, e1 ==> e1' -> srec e1 e2 e3 ==> srec e1' e2 e3
+| step_srec2 : forall e1 e2 e2' e3, e2 ==> e2' -> srec e1 e2 e3 ==> srec e1 e2' e3
+| step_srec3 : forall e1 e2 e3 e3', e3 ==> e3' -> srec e1 e2 e3 ==> srec e1 e2 e3'
+| step_srec_smk : forall e1 e2 e3 e4 e5, srec e1 e2 (smk e3 e4 e5) ==> e2 @ e4 @ e5
+
+| step_wt1 : forall e1 e1' e2, e1 ==> e1' -> wt e1 e2 ==> wt e1' e2
+| step_wt2 : forall e1 e2 e2', e2 ==> e2' -> wt e1 e2 ==> wt e1 e2'
+| step_sup1 : forall e1 e1' e2 e3, e1 ==> e1' -> sup e1 e2 e3 ==> sup e1' e2 e3
+| step_sup2 : forall e1 e2 e2' e3, e2 ==> e2' -> sup e1 e2 e3 ==> sup e1 e2' e3
+| step_sup3 : forall e1 e2 e3 e3', e3 ==> e3' -> sup e1 e2 e3 ==> sup e1 e2 e3'
+| step_wrec1 : forall e1 e1' e2 e3, e1 ==> e1' -> wrec e1 e2 e3 ==> wrec e1' e2 e3
+| step_wrec2 : forall e1 e2 e2' e3, e2 ==> e2' -> wrec e1 e2 e3 ==> wrec e1 e2' e3
+| step_wrec3 : forall e1 e2 e3 e3', e3 ==> e3' -> wrec e1 e2 e3 ==> wrec e1 e2 e3'
+| step_wrec_sup : forall e1 e2 e3 e4 e5, wrec e1 e2 (sup e3 e4 e5) 
+                                ==> e2 @ e4 @ (lam (e3 @ e4) (wrec (wk_deep 1 0 e1) (wk_deep 1 0 e2) (wk_deep 1 0 e5 @ &0)))
+
+| step_brec1 : forall e1 e1' e2 e3 e4, e1 ==> e1' -> brec e1 e2 e3 e4 ==> brec e1' e2 e3 e4
+| step_brec2 : forall e1 e2 e2' e3 e4, e2 ==> e2' -> brec e1 e2 e3 e4 ==> brec e1 e2' e3 e4
+| step_brec3 : forall e1 e2 e3 e3' e4, e3 ==> e3' -> brec e1 e2 e3 e4 ==> brec e1 e2 e3' e4
+| step_brec4 : forall e1 e2 e3 e4 e4', e4 ==> e4' -> brec e1 e2 e3 e4 ==> brec e1 e2 e3 e4'
+| step_brec_true : forall e1 e2 e3, brec e1 e2 e3 true ==> e2
+| step_brec_false : forall e1 e2 e3, brec e1 e2 e3 false ==> e3
+
+| step_urec1 : forall e1 e1' e2 e3, e1 ==> e1' -> urec e1 e2 e3 ==> urec e1' e2 e3
+| step_urec2 : forall e1 e2 e2' e3, e2 ==> e2' -> urec e1 e2 e3 ==> urec e1 e2' e3
+| step_urec3 : forall e1 e2 e3 e3', e3 ==> e3' -> urec e1 e2 e3 ==> urec e1 e2 e3'
+| step_urec_unit : forall e1 e2, urec e1 e2 unit ==> e2
+
+| step_exf1 : forall e1 e1' e2, e1 ==> e1' -> exf e1 e2 ==> exf e1' e2
+| step_exf2 : forall e1 e2 e2', e2 ==> e2' -> exf e1 e2 ==> exf e1 e2'
+where "a ==> b" := (step a b).
+
+Hint Constructors step par_red.
+
+Lemma step_par : forall e1 e2, e1 ==> e2 -> e1 ~> e2.
+  induction 1; eauto. Qed.
+
+Hint Resolve step_par.
+
+Ltac destr_sumors := match goal with [H: _ + {_} |- _] => destruct H end.
+Ltac destr_exists := match goal with [H: exists _,_ |- _] => destruct H | [H: {_ | _} |- _] => destruct H end.
+
+Require Import Relation_Definitions.
+Require Import Relation_Operators.
+
+(* typing will depend on evaluation, so preservation will have to wait until we've proved Church-Rosser *)
+
+Lemma wk_par_cong : forall e1 e2 n d, e1 ~> e2 -> wk_deep n d e1 ~> wk_deep n d e2.
+  intros e1 e2 n d He; generalize dependent d; generalize dependent n;
+  induction He; unfold wk_deep; simpl; intros; try (econstructor;eauto;fail); fold_ops.
+  (* lam_app and wrec, troublesome as always *)
+  - destruct d; [rewrite lift_subst_same_depth|rewrite lift_above_subst; [|omega]]; eauto.
+  - repeat rewrite wk_above_wk with (n1 := n) (d1 := S d); [|omega|omega|omega].
+    replace (wk_var n (S d) 0) with (&0) by auto; simpl; replace (d - 0) with d by omega.
+    eauto.
+Qed.  
+
+Hint Resolve wk_par_cong.
+
+Lemma par_eq : forall e1 e2 e3, e1 ~> e2 -> e2 = e3 -> e1 ~> e3.
+  induction 2; eauto. Qed.
+
+Lemma subst1_par_cong : forall e1 e2, e1 ~> e2 -> forall e3 n, e1 |> e3 // n ~> e2 |> e3 // n.
+  induction 1; unfold subst_deep; simpl; intros; fold_ops; eauto. 
+  - replace (subst_deep e0 n (subst_deep e5 0 e3)) with (subst_deep (subst_deep e0 n e5) 0 (subst_deep e0 (S n) e3));
+    [|rewrite subst_above_push]; eauto.
+  - replace (S n) with (1 + n); repeat rewrite <- lift_below_subst; eauto; omega.
+Qed.
+
+Lemma subst2_par_cong : forall e3 e1 e2 n, e1 ~> e2 -> e3 |> e1 // n ~> e3 |> e2 // n.
+  unfold subst_deep; induction e3; simpl; intros; try (econstructor;eauto;omega).
+  - unfold_ops; destr_choices; eauto.
+Qed.
+
+Hint Resolve subst1_par_cong subst2_par_cong.
+
+Lemma subst12_par_cong : forall e1 e2, e1 ~> e2 -> forall e3 e4 n, e3 ~> e4 -> e1 |> e3 // n ~> e2 |> e4 // n.
+  induction 1; unfold subst_deep; simpl; intros; fold_ops; try (unfold_ops; simpl in *; try econstructor; eauto; fail).
+  - eapply subst2_par_cong; eauto.
+  - rewrite subst_above_push; eauto.
+  - replace (S n) with (1 + n); repeat rewrite <- lift_below_subst; eauto; omega.
+Qed.
+
+Hint Resolve subst12_par_cong.
+
+Ltac notHyp P :=
+  match goal with
+    | [ _ : P |- _ ] => fail 1
+    | _ =>
+      match P with
+        | ?P1 /\ ?P2 => first [ notHyp P1 | notHyp P2 | fail 2 ]
+        | _ => idtac
+      end
+  end.
+
+Ltac extend pf :=
+  let t := type of pf in
+    notHyp t; generalize pf; intro.
+
+Ltac try_hyps := 
+  repeat match goal with
+           | [H: forall (e : ?T), _ , e : ?T |- _] => extend (H e)
+           | [IH: ?P -> _ , H: ?P |- _] => extend (IH H) 
+           | [IH: forall e, ?P e -> _ , H: ?P ?e |- _] => extend (IH e H)
+         end.
+
+Ltac clear_funs :=
+  repeat match goal with [H: forall e, _ |- _] => clear H | [H: _ -> _ |- _] => clear H end.
+
+Tactic Notation "test" tactic(tac) := tryif tac then fail "success" else fail "failure".
+Tactic Notation "not" tactic(tac) := tryif tac then fail else idtac.
+
+(** [atomic x] is the same as [idtac] if [x] is a variable or hypothesis, but is [fail 0] if [x] has internal structure. *)
+Ltac atomic x :=
+  match x with
+    | _ => is_evar x; fail 1 x "is not atomic (evar)"
+    | ?f _ => fail 1 x "is not atomic (application)"
+    | (fun _ => _) => fail 1 x "is not atomic (fun)"
+    | forall _, _ => fail 1 x "is not atomic (forall)"
+    | let x := _ in _ => fail 1 x "is not atomic (let in)"
+    | match _ with _ => _ end => fail 1 x "is not atomic (match)"
+    | _ => is_fix x; fail 1 x "is not atomic (fix)"
+    | context[?E] => (* catch-all *) (not constr_eq E x); fail 1 x "is not atomic (has subterm" E ")"
+    | _ => idtac
+  end.
+
+Ltac invert_atom_steps := 
+  repeat match goal with
+           | [H: ?e1 ~> ?e2 |- _] => atomic e2; (tryif atomic e1 then fail else (inversion H; subst; clear H))
+           | [H: ?e1 ==> ?e2 |- _] => atomic e2; (tryif atomic e1 then fail else (inversion H; subst; clear H))
+         end.
+
+Lemma par_diamond : forall e1 e2 e3, e1 ~> e2 -> e1 ~> e3 -> exists e4, e2 ~> e4 /\ e3 ~> e4.
+Proof with eauto.
+  intros e1 e2 e3 He2 He3; generalize dependent e3; induction He2; intros;
+  try (inversion He3; subst; try_hyps; clear_funs; destr_logic; eauto; fail).
+  - inversion He3; subst; try_hyps; clear_funs; destr_logic; invert_atom_steps; eauto.
+  - inversion He3; subst; try (try_hyps; clear_funs; destr_logic; invert_atom_steps; eauto; fail).
+    + specialize (IHHe2_1 _ H1); specialize (IHHe2_2 _ H3).
+      destruct IHHe2_1 as [e1' He1]; destruct IHHe2_2 as [e2' He2]; destr_logic.
+      inversion H2; subst; inversion H4; subst; eauto.
+  - inversion He3; subst; try (try_hyps; clear_funs; destr_logic; invert_atom_steps; eauto; fail).
+    + specialize (IHHe2_2 _ H3); specialize (IHHe2_3 _ H4); destr_logic; invert_atom_steps; eauto.
+      * exists (x0 @ e8 @ e9); eauto.
+      * exists (x0 @ e2'1 @ e3'0); eauto.
+  - inversion He3; subst; try (try_hyps; clear_funs; destr_logic; invert_atom_steps; eauto; fail).
+    + specialize (IHHe2_1 _ H4); specialize (IHHe2_2 _ H5); destr_logic; invert_atom_steps; eauto.
+      * exists (x0 @ e5 @ e6); eauto. 
+      * exists (x0 @ e2'1 @ e3'0); eauto.
+    + specialize (IHHe2_1 _ H3); specialize (IHHe2_2 _ H4); destr_logic; invert_atom_steps; eauto.
+      * exists (x0 @ e11 @ e12); inversion H; subst; split; eauto.
+      * exists (x0 @ e2'1 @ e3'); inversion H; subst; split; eauto.
+  - inversion He3; clear He3; subst; try (try_hyps; clear_funs; destr_logic; invert_atom_steps; eauto; fail).
+    + specialize (IHHe2_1 _ H2); specialize (IHHe2_2 _ H4); specialize (IHHe2_3 _ H5).
+      destruct IHHe2_1 as [e1'' He1], IHHe2_2 as [e2'' He2], IHHe2_3 as [e3'' He3].
+      destr_logic; invert_atom_steps; eexists; (split; [eapply par_wrec_sup; eassumption|]); repeat econstructor; eauto.
+  - inversion He3; clear He3; subst; try (try_hyps; clear_funs; destr_logic; invert_atom_steps; eauto; fail).
+    + specialize (IHHe2_1 _ H2); specialize (IHHe2_2 _ H4); specialize (IHHe2_3 _ H5).
+      destruct IHHe2_1 as [e1'' He1]; destruct IHHe2_2 as [e2'' He2]; destruct IHHe2_3 as [e3'' He3];
+      destr_logic; invert_atom_steps;
+      eexists; (split; [|eapply par_wrec_sup; eassumption]); repeat econstructor; try apply wk_par_cong; assumption.
+    + specialize (IHHe2_1 _ H2); specialize (IHHe2_2 _ H4); specialize (IHHe2_3 _ H5);
+      destruct IHHe2_1 as [e1'' He1]; destruct IHHe2_2 as [e2'' He2]; destruct IHHe2_3 as [e3'' He3];
+      destruct He3 as [He31 He32]; inversion He31; subst; inversion He32; subst; destr_logic;
+      eexists; split; repeat (eapply par_app || eapply par_lam || eapply par_wrec);
+      try apply wk_par_cong; try eassumption; eauto.
+  - inversion He3; clear He3; subst; try (try_hyps; clear_funs; destr_logic; invert_atom_steps; eauto; fail);
+    try_hyps; clear_funs; destr_logic; 
+    match goal with [H: true ~> _ |- _] => inversion H; subst | [H: false ~> _ |- _] => inversion H; subst end; eauto.
+  - inversion He3; clear He3; subst; try_hyps; clear_funs; destr_logic; invert_atom_steps; eauto;
+    repeat match goal with [H: true ~> _ |- _] => inversion H; subst; clear H | [H: false ~> _ |- _] => inversion H; subst; clear H end;
+    eauto.
+  - inversion He3; clear He3; subst; try_hyps; clear_funs; destr_logic; invert_atom_steps; eauto;
+    repeat match goal with [H: true ~> _ |- _] => inversion H; subst; clear H | [H: false ~> _ |- _] => inversion H; subst; clear H end;
+    eauto.
+  - inversion He3; clear He3; subst; try_hyps; clear_funs; destr_logic; invert_atom_steps; eauto;
+    repeat match goal with [H: unit ~> _ |- _] => inversion H; subst end; eauto.
+  - inversion He3; clear He3; subst; try_hyps; clear_funs; destr_logic; invert_atom_steps; eauto;
+    repeat match goal with [H: unit ~> _ |- _] => inversion H; subst; clear H end; eauto.
+Qed.
+
+Infix "~~>" := (clos_trans exp par_red) (at level 50).
+Hint Constructors clos_trans.
+
+Hint Resolve par_diamond.
+
+Lemma par_left_fill : forall e1 e2 e3, e1 ~> e2 -> e1 ~~> e3 -> exists e4, e2 ~~> e4 /\ e3 ~> e4.
+  intros e1 e2 e3 He2 He3; generalize dependent e2; induction He3; intros.
+  - destruct (par_diamond H He2); destr_logic; eauto.
+  - try_hyps; destr_logic; try_hyps; destr_logic; eauto.
+Qed.
+
+Lemma par_confluent : forall e1 e2 e3, e1 ~~> e2 -> e1 ~~> e3 -> exists e4, e2 ~~> e4 /\ e3 ~~> e4.
+  intros e1 e2 e3 He2 He3; generalize dependent e3; induction He2; intros.
+  - destruct (par_left_fill H He3); destr_logic; eauto.
+  - try_hyps; destr_logic; try_hyps; destr_logic; eauto.
+ Qed.
+
+Infix "===>" := (clos_refl_trans_1n exp step) (at level 50).
+Hint Constructors clos_refl_trans_1n.
+
+Lemma rtc_rtc : forall A R e1 e2 e3, clos_refl_trans_1n A R e1 e2 -> clos_refl_trans_1n A R e2 e3 -> clos_refl_trans_1n A R e1 e3.
+  induction 1; eauto. Qed.
+
+Lemma pi_rtc_cong : forall e1 e1', e1 ===> e1' -> forall e2 e2', e2 ===> e2' -> pi e1 e2 ===> pi e1' e2'.
+  repeat induction 1; intros; eauto; eapply rtc_rtc; eauto. Qed.
+
+Lemma lam_rtc_cong : forall e1 e1', e1 ===> e1' -> forall e2 e2', e2 ===> e2' -> lam e1 e2 ===> lam e1' e2'.
+  repeat induction 1; intros; eauto; eapply rtc_rtc; eauto. Qed.
+
+Lemma app_rtc_cong : forall e1 e1', e1 ===> e1' -> forall e2 e2', e2 ===> e2' -> app e1 e2 ===> app e1' e2'.
+  repeat induction 1; intros; eauto; eapply rtc_rtc; eauto. Qed.
+
+Lemma sg_rtc_cong : forall e1 e1', e1 ===> e1' -> forall e2 e2', e2 ===> e2' -> sigma e1 e2 ===> sigma e1' e2'.
+  repeat induction 1; intros; eauto; eapply rtc_rtc; eauto. Qed.
+
+Lemma smk_rtc_cong : forall e1 e1', e1 ===> e1' -> forall e2 e2', e2 ===> e2' -> forall e3 e3', e3 ===> e3' -> smk e1 e2 e3 ===> smk e1' e2' e3'.
+  repeat induction 1; intros; eauto; eapply rtc_rtc; eauto. Qed.
+
+Lemma srec_rtc_cong : forall e1 e1', e1 ===> e1' -> forall e2 e2', e2 ===> e2' -> forall e3 e3', e3 ===> e3' -> srec e1 e2 e3 ===> srec e1' e2' e3'.
+  repeat induction 1; intros; eauto; eapply rtc_rtc; eauto. Qed.
+
+Lemma wt_rtc_cong : forall e1 e1', e1 ===> e1' -> forall e2 e2', e2 ===> e2' -> wt e1 e2 ===> wt e1' e2'.
+  repeat induction 1; intros; eauto; eapply rtc_rtc; eauto. Qed.
+
+Lemma sup_rtc_cong : forall e1 e1', e1 ===> e1' -> forall e2 e2', e2 ===> e2' -> forall e3 e3', e3 ===> e3' -> sup e1 e2 e3 ===> sup e1' e2' e3'.
+  repeat induction 1; intros; eauto; eapply rtc_rtc; eauto. Qed.
+
+Lemma wrec_rtc_cong : forall e1 e1', e1 ===> e1' -> forall e2 e2', e2 ===> e2' -> forall e3 e3', e3 ===> e3' -> wrec e1 e2 e3 ===> wrec e1' e2' e3'.
+  repeat induction 1; intros; eauto; eapply rtc_rtc; eauto. Qed.
+
+Lemma urec_rtc_cong : forall e1 e1', e1 ===> e1' -> forall e2 e2', e2 ===> e2' -> forall e3 e3', e3 ===> e3' -> urec e1 e2 e3 ===> urec e1' e2' e3'.
+  repeat induction 1; intros; eauto; eapply rtc_rtc; eauto. Qed.
+
+Lemma brec_rtc_cong : forall e1 e1', e1 ===> e1' -> forall e2 e2', e2 ===> e2' ->
+                      forall e3 e3', e3 ===> e3' -> forall e4 e4', e4 ===> e4' -> brec e1 e2 e3 e4 ===> brec e1' e2' e3' e4'.
+  repeat induction 1; intros; eauto; eapply rtc_rtc; eauto. Qed.
+
+Lemma exf_rtc_cong : forall e1 e1', e1 ===> e1' -> forall e2 e2', e2 ===> e2' -> exf e1 e2 ===> exf e1' e2'.
+  repeat induction 1; intros; eauto; eapply rtc_rtc; eauto. Qed.
+
+Hint Resolve pi_rtc_cong lam_rtc_cong app_rtc_cong sg_rtc_cong smk_rtc_cong srec_rtc_cong.
+Hint Resolve wt_rtc_cong sup_rtc_cong wrec_rtc_cong urec_rtc_cong brec_rtc_cong exf_rtc_cong.
+
+Lemma par_step_rtc : forall e1 e2, e1 ~> e2 -> e1 ===> e2.
+  induction 1; eauto; eapply rtc_rtc;
+  [eapply app_rtc_cong| |eapply srec_rtc_cong| |eapply wrec_rtc_cong| |
+   eapply brec_rtc_cong| |eapply brec_rtc_cong| |eapply urec_rtc_cong|];
+  eauto. Qed.
+
+Hint Resolve par_step_rtc.
+
+Lemma step_rtc_equiv : forall e1 e2, e1 ~~> e2 <-> e1 ===> e2.
+  split; induction 1; eauto. eapply rtc_rtc; eauto. Qed.
+
+Hint Resolve step_rtc_equiv.
+
+Lemma step_confluent : forall e1 e2 e3, e1 ===> e2 -> e1 ===> e3 -> exists e4, e2 ===> e4 /\ e3 ===> e4.
+  intros e1 e2 e3 H1 H2. 
+  apply step_rtc_equiv in H1; apply step_rtc_equiv in H2.
+  destruct (par_confluent H1 H2) as [x H]; destruct H.
+  exists x; split; apply step_rtc_equiv; eauto.
+Qed.
+
+Lemma step_pi_pi e1 e2 e3 : pi e1 e2 ==> e3 -> exists e4 e5, e3 = pi e4 e5.
+  inversion 1; eauto. Qed.
+
+Ltac invert_nonatomics :=
+  repeat match goal with [H: ?e1 = ?e2 |- _] => tryif (atomic e1 || atomic e2) then fail else inversion H; subst; clear H end.
+
+Lemma eval_pi_pi e1 e2 e3 (p : pi e1 e2 ===> e3) : exists e4 e5, e3 = pi e4 e5 /\ e1 ===> e4 /\ e2 ===> e5.
+  remember (pi e1 e2) as p12; generalize dependent e2; generalize dependent e1.
+  induction p; intros; subst; [eauto|].
+  - inversion H; subst.
+    + specialize (IHp e1' e2 eq_refl); destr_logic; subst; repeat eexists; eauto.
+    + specialize (IHp e1 e2' eq_refl); destr_logic; subst; repeat eexists; eauto.
+Qed.
+
+Lemma eval_lam_lam e1 e2 e3 (p : lam e1 e2 ===> e3) : exists e4 e5, e3 = lam e4 e5 /\ e1 ===> e4 /\ e2 ===> e5.
+  remember (lam e1 e2) as p12; generalize dependent e2; generalize dependent e1.
+  induction p; intros; subst; [eauto|].
+  - inversion H; subst.
+    + specialize (IHp e1' e2 eq_refl); destr_logic; subst; repeat eexists; eauto.
+    + specialize (IHp e1 e2' eq_refl); destr_logic; subst; repeat eexists; eauto.
+Qed.
+
+Lemma eval_sg_sg e1 e2 e3 (p : sigma e1 e2 ===> e3) : exists e4 e5, e3 = sigma e4 e5 /\ e1 ===> e4 /\ e2 ===> e5.
+  remember (sigma e1 e2) as p12; generalize dependent e2; generalize dependent e1.
+  induction p; intros; subst; [eauto|].
+  - inversion H; subst.
+    + specialize (IHp e1' e2 eq_refl); destr_logic; subst; repeat eexists; eauto.
+    + specialize (IHp e1 e2' eq_refl); destr_logic; subst; repeat eexists; eauto.
+Qed.
+
+Lemma eval_wt_wt e1 e2 e3 (p : wt e1 e2 ===> e3) : exists e4 e5, e3 = wt e4 e5 /\ e1 ===> e4 /\ e2 ===> e5.
+  remember (wt e1 e2) as p12; generalize dependent e2; generalize dependent e1.
+  induction p; intros; subst; [eauto|].
+  - inversion H; subst.
+    + specialize (IHp e1' e2 eq_refl); destr_logic; subst; repeat eexists; eauto.
+    + specialize (IHp e1 e2' eq_refl); destr_logic; subst; repeat eexists; eauto.
+Qed.
+
+Lemma eval_exf_exf e1 e2 e3 (p : exf e1 e2 ===> e3) : exists e4 e5, e3 = exf e4 e5 /\ e1 ===> e4 /\ e2 ===> e5.
+  remember (exf e1 e2) as p12; generalize dependent e2; generalize dependent e1.
+  induction p; intros; subst; [eauto|].
+  - inversion H; subst.
+    + specialize (IHp e1' e2 eq_refl); destr_logic; subst; repeat eexists; eauto.
+    + specialize (IHp e1 e2' eq_refl); destr_logic; subst; repeat eexists; eauto.
+Qed.
+
+Lemma eval_smk_smk e1 e2 e3 e4 (p : smk e1 e2 e3 ===> e4) : exists e5 e6 e7, e4 = smk e5 e6 e7 /\ e1 ===> e5 /\ e2 ===> e6 /\ e3 ===> e7.
+  remember (smk e1 e2 e3) as p12; generalize dependent e3; generalize dependent e2; generalize dependent e1.
+  induction p; intros; subst; [repeat eexists; eauto|].
+  - inversion H; subst.
+    + specialize (IHp e1' e2 e3 eq_refl); destr_logic; subst; repeat eexists; eauto.
+    + specialize (IHp e1 e2' e3 eq_refl); destr_logic; subst; repeat eexists; eauto.
+    + specialize (IHp e1 e2 e3' eq_refl); destr_logic; subst; repeat eexists; eauto.
+Qed.
+
+Lemma eval_sup_sup e1 e2 e3 e4 (p : sup e1 e2 e3 ===> e4) : exists e5 e6 e7, e4 = sup e5 e6 e7 /\ e1 ===> e5 /\ e2 ===> e6 /\ e3 ===> e7.
+  remember (sup e1 e2 e3) as p12; generalize dependent e3; generalize dependent e2; generalize dependent e1.
+  induction p; intros; subst; [repeat eexists; eauto|].
+  - inversion H; subst.
+    + specialize (IHp e1' e2 e3 eq_refl); destr_logic; subst; repeat eexists; eauto.
+    + specialize (IHp e1 e2' e3 eq_refl); destr_logic; subst; repeat eexists; eauto.
+    + specialize (IHp e1 e2 e3' eq_refl); destr_logic; subst; repeat eexists; eauto.
+Qed.
+
+Definition is_normal e : Prop := forall e', ~ e ==> e'.
+
+Hint Unfold is_normal.
+
+Theorem normal_forms_unique : forall e1 e2 e3, is_normal e2 -> is_normal e3 -> e1 ===> e2 -> e1 ===> e3 -> e2 = e3.
+  intros e1 e2 e3 He2 He3 Hs1 Hs2.
+  assert (H: exists e4, e2 ===> e4 /\ e3 ===> e4) by (apply step_confluent with (e1 := e1); auto).
+  destruct H as [e4 He4]; destruct He4 as [Hc1 Hc2]; destruct Hc1; destruct Hc2; auto;
+  unfold is_normal in *; try_hyps; contradiction.
+Qed.
