coq-in-coq/Scoping.v
@@ -1,0 +1,287 @@
+Require Export Unscoped Evaluation.
+Require Import Omega.
+
+(* Scoping relation and DeBrujin lemmas live here *)
+Inductive scoped_at (n : nat) : exp -> Prop :=
+| scope_var : forall i, i < n -> scoped_at n (& i)
+
+| scope_typ : forall m, scoped_at n (typ m)
+
+| scope_pi : forall a b, scoped_at n a -> scoped_at (S n) b -> scoped_at n (pi a b)
+| scope_lam : forall A b, scoped_at n A -> scoped_at (S n) b -> scoped_at n (lam A b)
+| scope_app : forall f x, scoped_at n f -> scoped_at n x -> scoped_at n (f @ x)
+
+| scope_sigma : forall a b, scoped_at n a -> scoped_at n b -> scoped_at n (sigma a b)
+| scope_smk : forall B a b, scoped_at n B -> scoped_at n a -> scoped_at n b -> scoped_at n (smk B a b)
+| scope_srec : forall c p s, scoped_at n c -> scoped_at n p -> scoped_at n s -> scoped_at n (srec c p s)
+
+| scope_wt : forall a b, scoped_at n a -> scoped_at n b -> scoped_at n (wt a b)
+| scope_sup : forall B a f, scoped_at n B -> scoped_at n a -> scoped_at n f -> scoped_at n (sup B a f)
+| scope_wrec : forall c s w, scoped_at n c -> scoped_at n s -> scoped_at n w -> scoped_at n (wrec c s w)
+
+| scope_bool : scoped_at n bool
+| scope_true : scoped_at n true
+| scope_false : scoped_at n false
+| scope_brec : forall c t f b, scoped_at n c -> scoped_at n t -> scoped_at n f -> scoped_at n b -> scoped_at n (brec c t f b)
+
+| scope_top : scoped_at n top
+| scope_unit : scoped_at n unit
+| scope_urec : forall c u t, scoped_at n c -> scoped_at n u -> scoped_at n t -> scoped_at n (urec c u t)
+
+| scope_bot : scoped_at n bot
+| scope_exf : forall c f, scoped_at n c -> scoped_at n f -> scoped_at n (exf c f).
+
+Hint Resolve lt_dec.
+
+Hint Constructors scoped_at.
+Hint Constructors sumbool.
+
+Definition scope_check_at (n : nat) (e : exp) : {scoped_at n e} + {~ scoped_at n e}.
+  (* Local Hint Extern 5 => match goal with [H : scoped_at _ _ |- _] => inversion H end. *)
+  generalize dependent n; induction e; intro n;
+  try (destruct (lt_dec ix n); [left|right]; auto; inversion 1; auto);
+  Inster_all; destr_sums; try (left; constructor; eassumption); right; inversion 1; subst; auto.
+Defined.
+
+Fixpoint count_free (e : exp) : nat :=
+  match e with
+    | & i => S i
+
+    | pi a b => max (count_free a) (pred (count_free b))
+    | lam A b => max (count_free A) (pred (count_free b))
+    | (f @ x) => max (count_free f) (count_free x)
+
+    | sigma a b => max (count_free a) (count_free b)
+    | (smk B a b) => max (max (count_free B) (count_free a)) (count_free b)
+    | srec c p s => max (max (count_free c) (count_free p)) (count_free s)
+
+    | wt a b => max (count_free a) (count_free b)
+    | sup B a f => max (max (count_free B) (count_free a)) (count_free f)
+    | wrec c s w => max (max (count_free c) (count_free s)) (count_free w)
+
+    | brec c t f b => max (max (max (count_free c) (count_free t)) (count_free f)) (count_free b)
+    | urec c u t => max (max (count_free c) (count_free u)) (count_free t)
+    | exf c f => max (count_free c) (count_free f)
+    
+    | _ => 0
+  end.
+
+Lemma scoped_at_lift (e : exp) n (p : scoped_at n e) : forall m, n <= m -> scoped_at m e.
+  induction p; intros; constructor; try apply IHp; try apply IHp1; try apply IHp2; try apply IHp3; try apply IHp4; omega.
+Qed.
+
+Hint Resolve scoped_at_lift.
+Hint Resolve Nat.le_max_l Nat.le_max_r.
+
+Hint Extern 1 (?n <= max ?n ?m) => apply Nat.le_max_l.
+
+Lemma le_S_pred : forall n, n <= S (pred n). intro; omega. Qed.
+Lemma S_max_pred : forall n m, S (max n m) = max (S n) (S m). induction n; induction m; auto. Qed.
+
+Hint Rewrite S_max_pred.
+
+Ltac SMax := repeat match goal with
+                      | [ |- context[S (max _ _)] ] => rewrite S_max_pred
+                    end.
+
+Lemma max_trans_l : forall d n m, d <= n -> d <= max n m. intros; eapply le_trans; eauto. Qed.
+Lemma max_trans_r : forall d n m, d <= m -> d <= max n m. intros; eapply le_trans; eauto. Qed.
+
+Hint Resolve max_trans_l max_trans_r.
+Ltac le_max :=
+  match goal with
+    | [|- ?d <= max ?n ?m] => (eapply max_trans_l; try le_max; omega; fail) || (eapply max_trans_r; try le_max; omega; fail)
+  end.
+Theorem scoped_at_count (e : exp) : scoped_at (count_free e) e.
+  Local Hint Resolve le_n_S.
+  Local Hint Resolve le_S_pred.
+  Local Hint Extern 1 => SMax.
+  induction e; intros;
+  try (constructor; simpl in *; omega);
+  try (constructor; simpl; SMax; (eapply scoped_at_lift; [eassumption|le_max])).
+Qed.
+
+Lemma max_le_eq_l : forall n m, n <= m -> max n m = m.
+  induction n; induction m; inversion 1; subst; simpl; eauto.
+  - f_equal; apply IHn; omega.
+Qed.
+
+Lemma max_le_eq_r : forall n m, n <= m -> max m n = m.
+  induction n; induction m; inversion 1; subst; simpl; eauto.
+  - f_equal; apply IHn; omega.
+Qed.
+
+Lemma max_refl : forall n, max n n = n. intros; apply max_le_eq_l; eauto. Qed.
+
+Hint Rewrite max_le_eq_l max_le_eq_r max_refl.
+Local Hint Resolve max_le_eq_l max_le_eq_r max_refl.
+
+Lemma max_left_right : forall n m, (max n m = n) \/ (max n m = m).
+  intros; destruct (lt_eq_lt_dec n m) as [Hle|Hgt]; [destruct Hle as [Hlt|Heq]|]; subst;
+  [right;apply max_le_eq_l|right;apply max_refl|left;apply max_le_eq_r]; omega. Qed.
+
+Lemma max_le_trans : forall n m d, n <= d -> m <= d -> max n m <= d.
+  intros; destruct (max_left_right n m) as [Hn|Hm]; [rewrite Hn|rewrite Hm]; eauto. Qed.
+
+Local Hint Resolve max_le_trans.
+
+(* well, at least this was easy *)
+Theorem count_free_least (e : exp) : forall n, scoped_at n e -> count_free e <= n.
+  induction 1; simpl in *; repeat apply max_le_trans; omega. Qed.
+
+(* Weaking and Subst lemmas *)
+Theorem wk_scoped (e : exp) n (p : scoped_at n e) : forall m d, scoped_at (m + n) (wk_deep m d e).
+  induction p; intros; unfold wk_deep in *; simpl; try constructor; simpl; repeat rewrite plus_n_Sm; auto.
+  - unfold wk_var; simpl; destruct (le_dec d i); constructor; omega.
+Qed.
+
+Hint Resolve wk_scoped.
+
+Lemma wk_0_scoped e m n (p : scoped_at n e) : scoped_at (m + n) (wk_deep m 0 e). auto. Qed.
+Lemma wk_1_scoped e n (p : scoped_at n e) : scoped_at (S n) (wk_deep 1 0 e). replace (S n) with (1 + n) by auto; auto. Qed.
+
+Lemma subst_scoped_pred (e : exp) n (p : scoped_at n e) :
+  forall d v, d < n -> scoped_at (n - S d) v -> scoped_at (pred n) (e |> v // d).
+  induction p; intros d v Hd Hv; (destruct n; simpl in *; [exfalso;omega|]);
+  try constructor;
+  (* try applying all the IH's *)
+  try (apply IHp; [omega|auto]); try (apply IHp1; [omega|auto]);
+  try (apply IHp2; [omega|auto]); try (apply IHp3; [omega|auto]); try (apply IHp4; [omega|auto]).
+  (* vars, the always special case *)
+  - unfold subst_deep; unfold subst_var; simpl; destruct (lt_eq_lt_dec i d) as [Hle|Hgt]; [destruct Hle as [Hlt|_]|];
+    [constructor|replace n with (d + (n - d)) by omega; apply wk_scoped|constructor]; [omega|auto|omega].
+Qed.
+
+Theorem subst_scoped (e : exp) n (p : scoped_at (S n) e) :
+  forall d v, d <= n -> scoped_at (n - d) v -> scoped_at n (e |> v // d).
+  replace n with (pred (S n)) by omega; intros; apply subst_scoped_pred; auto. Qed.
+
+Hint Resolve subst_scoped.
+
+Theorem subst_0_scoped (e : exp) n (p : scoped_at (S n) e) v : scoped_at n v -> scoped_at n (e |> v // 0).
+  intro H. replace n with (n - 0) in H by omega. apply subst_scoped; auto; omega. Qed.
+
+Definition con := list exp.
+Open Scope list_scope.
+
+Inductive scoped_con : con -> Prop :=
+| scope_nil : scoped_con nil
+| scope_cons : forall Gamma X, scoped_con Gamma -> scoped_at (length Gamma) X -> scoped_con (X :: Gamma).
+
+Hint Constructors scoped_con.
+
+Lemma unwk_scoped : forall e n m d, d <= m -> scoped_at (n + m) (wk_deep n d e) -> scoped_at m e.
+  induction e; intros n m d Hd He; simpl in *; try (
+  (* dispatch trivial cases *)
+  try (repeat constructor; auto; fail);
+  (* var case takes some special handling *)
+  try (unfold wk_deep in *; unfold wk_var in *; simpl in *; destruct (le_dec d ix));
+  (* invert and split obligations *)
+  inversion He; subst; constructor; simpl in *; repeat rewrite plus_n_Sm in *;
+  (* try all the IH's *)
+  try eapply (IHe1 n); try eapply (IHe2 n); try eapply (IHe3 n); try eapply (IHe4 n);
+  (* finish the job *)
+  try eassumption; omega).
+Qed.
+
+Hint Resolve unwk_scoped.
+
+Lemma unsubst_scoped : forall e v d n, d <= n -> scoped_at (n - d) v -> scoped_at n (e |> v // d) -> scoped_at (S n) e.
+  induction e; intros v d n Hd Hv He; unfold subst_deep in *; simpl in *;
+  (* var case always takes some special care *)
+  try (unfold subst_var in *; simpl in *;
+       destruct (lt_eq_lt_dec ix d) as [Hle|Hgt]; [destruct Hle as [Hlt|Heq]|]; inversion He; constructor; omega);
+  (* invert things and split *)
+  inversion He; subst; repeat constructor;
+  (* try all IH's *)
+  try eapply (IHe v); try eapply (IHe1 v); try eapply (IHe2 v); try eapply (IHe3 v); try eapply (IHe4 v);
+  match goal with
+    (* use ordering cases to instantiate d *)
+    | [|- _ <= _] => repeat (try apply Hd; apply le_n_S in Hd)
+    | _ => assumption (* otherwise it'll just be a piece of He *)
+ end.
+Qed.
+
+Lemma unsubst_0_scoped : forall e v n, scoped_at n v -> scoped_at n (e |> v // 0) -> scoped_at (S n) e.
+  intros e v n Hv He; apply unsubst_scoped in He; try rewrite <- minus_n_O; try assumption; omega. Qed.
+
+Lemma wk_above_scope : forall e n1 n2 d, n1 <= d -> scoped_at n1 e -> wk_deep n2 d e = e.
+  intros e n1 n2 d Hd He; generalize dependent n2; generalize dependent d; induction He;
+  unfold wk_deep; simpl; try reflexivity; intros; fold_ops; f_equal; auto; try omega.
+  - unfold_ops; simpl; destr_choices; f_equal; omega.
+Qed.
+
+Lemma subst_above_scope : forall e n v d, n <= d -> scoped_at n e -> e |> v // d = e.
+  intros e n1 n2 d Hd He; generalize dependent n2; generalize dependent d; induction He;
+  unfold subst_deep; simpl; try reflexivity; intros; fold_ops; f_equal; auto; try omega.
+  - unfold_ops; simpl; destr_choices; f_equal; omega.
+Qed.
+
+(* Evaluation preserves scope *)
+Ltac invert_atom_scopes :=
+  repeat match goal with [H: scoped_at _ ?e |- _] => tryif atomic e then fail else (inversion H; subst; clear H) end.
+
+Theorem step_scoped : forall e1 e2, e1 ==> e2 -> forall n, scoped_at n e1 -> scoped_at n e2.
+  induction 1; auto; intros; invert_atom_scopes; try_hyps; repeat (constructor;(omega || auto));
+  try apply subst_0_scoped; try apply wk_1_scoped; assumption.
+Qed.
+
+Theorem eval_scoped : forall e1 e2, e1 ===> e2 -> forall n, scoped_at n e1 -> scoped_at n e2.
+  induction 1; auto; intros n Hn.
+  - apply IHclos_refl_trans_1n; eapply step_scoped; eauto.
+Qed.
+
+(*
+Require Import TypeChecking.
+
+Theorem typed_implies_scoped : forall Gamma t T, scoped_con Gamma -> Gamma ⊢ t ∈ T -> scoped_at (length Gamma) T /\ scoped_at (length Gamma) t.
+Proof with try eassumption.
+  intros Gamma t T Hg.
+  induction 1; auto; simpl in *; try (repeat constructor; auto; fail);
+  try (destruct (IHhas_type Hg) as [IH1 IH2]);
+  try (destruct (IHhas_type1 Hg) as [IH11 IH12]); try (destruct (IHhas_type2 Hg) as [IH21 IH22]);
+  try (destruct (IHhas_type3 Hg) as [IH31 IH32]); try (destruct (IHhas_type4 Hg) as [IH41 IH42]);
+  try (destruct (IHhas_type2 (scope_cons _ _ Hg IH12)) as [IH21 IH22]);
+  try (split; repeat constructor; auto; fail).
+  (* app is weird *)
+  - split; try (constructor; auto).
+    + inversion IH11; subst; apply subst_0_scoped...
+  - split; try (constructor; auto); (eapply unsubst_scoped_O; [|eassumption])...
+  (* recursion principles will take special handling *)
+  - inversion IH21; subst. assert (Hg' : scoped_con (B :: A :: Gamma)) by auto. destruct (IHhas_type1 Hg') as [IH11 IH12].
+    assert (IHC : scoped_at (S(length Gamma)) C).
+      + apply unwk_scoped with (n := 2) (d := 1); [omega|eapply unsubst_scoped_O]; [|eassumption].
+        * constructor; [eapply scoped_at_lift; [eassumption|]; omega| |]; constructor; omega.
+      + split; [eapply subst_0_scoped; auto|constructor]...
+  (* oh, and so will sup *)
+  - destruct (IHhas_type2 (scope_cons _ _ Hg IH11)) as [IH21 IH22].
+    assert (Hg'' : scoped_con (subst_deep a 0 B :: Gamma)).
+      constructor; [|apply subst_0_scoped]...
+    destruct (IHhas_type3 Hg''); split; auto.
+  (* now for the /really/ fun one, wrec *)
+  - inversion IH21; subst.
+    assert (Hg' : scoped_con (wk_at 1 B :: pi B (wk_deep 2 0 (wt A B)) :: A :: Gamma)).
+      constructor; [constructor ;[constructor|]|];
+      [| |simpl; constructor; try assumption;
+          replace (S (S (length Gamma))) with (2 + length Gamma) by omega;
+          apply wk_scoped; constructor
+       | simpl; replace (S (S (length Gamma))) with (1 + S(length Gamma)) by omega; apply wk_scoped]...
+    destruct (IHhas_type1 Hg') as [IH11 IH12].
+    assert (Hc : scoped_at (S (length Gamma)) C). 
+      apply unsubst_scoped_O in IH11; [|constructor;constructor;omega].
+      apply unwk_scoped with (n := 3) (d := 1); [omega|]...
+    split; [apply subst_0_scoped|constructor]...
+  - assert (Hc : scoped_at (S (length Gamma)) C).
+      eapply unsubst_scoped_O; [|eassumption]; auto.
+    split; [apply subst_0_scoped|constructor]...
+  - assert (Hc : scoped_at (S (length Gamma)) C).
+      eapply unsubst_scoped_O; [|eassumption]; auto.
+    split; [apply subst_0_scoped|constructor]...
+  - destruct (IHhas_type1 (scope_cons _ _ Hg (scope_bot _))) as [IH11 IH12].
+    split; [apply subst_0_scoped|constructor]...
+Qed. (* seems like it ought to be possible to automate more of that, but for now I'll just leave it be *)
+
+Theorem wf_implies_scoped : forall Gamma, wf_con Gamma -> scoped_con Gamma.
+  induction 1; constructor; try eapply typed_implies_scoped; eassumption. Qed.
+
+Lemma typ_uq Gamma e T1 T2 : Gamma ⊢ e ∈ T1 -> Gamma ⊢ e ∈ T2 -> T1 = T2. *)
